layout trimming, and a para on prefxes.

2022-ITP-TQM/paper.thy
@@ -120,7 +120,6 @@ term\<open>4500\<close>
 declare[[show_sorts=false]]
 
 thm metre_definition kilogram_definition
-
 (*>*)
 text\<open>
 As a result of our theory development\<^footnote>\<open>The sources can be found 
@@ -150,10 +149,8 @@ reconciled, however, and so some substantial theory engineering is required. On 
 we want a deep integration of dimensions and units into the Isabelle type system. On the
 other, we need to do normal-form calculations on types, so that, for example, the units 
 \<^typ>\<open>'\<alpha>[s \<cdot> m \<cdot> s\<^sup>-\<^sup>2]\<close> and \<^typ>\<open>'\<alpha>[m \<cdot> s\<^sup>-\<^sup>1]\<close> can be equated.
-\<close>
 
-text\<open>
-Isabelle's type system follows the Curry-style paradigm, which rules out the possibility of direct 
+Isabelle's type system follows the Curry-style paradigm, which rules out the possibility of direct
 calculations on type-terms (in contrast to Coq-like systems). However, our semantic interpretation 
 of ISQ and SI requires the foundation of the heterogeneous equivalence relation \<open>\<cong>\<^sub>Q\<close> 
 in semantic terms. This means that we can relate quantities with syntactically different dimension 
@@ -161,22 +158,9 @@ types, yet with same dimension semantics. This paves the way for derived rules t
 of terms, which represent type computations indirectly. This principle is the basis for the tactic 
 support, which allows for the dimensional type checking of key definitions of the SI system
 inside Isabelle/HOL, \<^ie> without making use of code-generated reflection. 
-For example, the crucial definitions adapted from the SI Brochure that 
-give the concrete definitions for the metre and the kilogram can be presented as follows: \<^vs>\<open>0.3cm\<close>
+The resulting proof-support allows for an automatic check of physical equations
+such as those defining SI units.\<close>
 
-\<^theory_text>\<open>theorem metre_definition\<close>
-\<^item> @{term [show_types=false]\<open>1 *\<^sub>Q metre \<cong>\<^sub>Q \<^bold>c \<^bold>\<cdot> (299792458 *\<^sub>Q \<one>)\<^sup>-\<^sup>\<one> \<^bold>\<cdot> second\<close>}
-\<^item> @{term [show_types=false]\<open>1 *\<^sub>Q metre \<cong>\<^sub>Q 9192631770 / 299792458 *\<^sub>Q \<^bold>c \<^bold>\<cdot> (9192631770 *\<^sub>Q second\<^sup>-\<^sup>\<one>)\<^sup>-\<^sup>\<one>\<close>}
-
-\<^noindent> \<^theory_text>\<open>theorem kilogram_definition\<close>
-\<^item> \<^term>\<open>((1 *\<^sub>Q kilogram)::('\<alpha>::field_char_0) kilogram) \<cong>\<^sub>Q (\<^bold>h \<^bold>/ (6.62607015 \<cdot> 1/(10^34) *\<^sub>Q \<one>))\<^bold>\<cdot>metre\<^sup>-\<^sup>\<two>\<^bold>\<cdot>second\<close> 
-\<close>
-
-text\<open>
-These equations give the concrete definitions for the 
-metre and kilogram in terms of the physical constants \<^term>\<open>\<^bold>c\<close> (speed of light) and \<^term>\<open>\<^bold>h\<close> 
-(Planck constant). They can be proven directly using the tactic \<^theory_text>\<open>si-calc\<close> provided by our theory.
-\<close>
 
 (*<*)
 declare_reference*[induct_type_set::figure]
@@ -216,11 +200,11 @@ Our ISQ and SI model provides the following fundamental concepts:
   as \<open>m\<close>, \<open>kg\<close>, \<open>s\<close>, \<open>A\<close>, \<open>K\<close>,  \<open>mol\<close>, and  \<open>cd\<close>.
 
 \<^enum> a standardised set of symbols of SI-prefixes for multiples of SI-units, such as
-  \<^term>\<open>giga\<close> (\<open>=10\<^sup>9\<close>), \<^term>\<open>kilo\<close> (\<open>=10\<^sup>3\<close>),  \<^term>\<open>milli\<close> (\<open>=10\<^sup>-\<^sup>3\<close>), etc.
+  \<^term>\<open>giga\<close> (\<open>=10\<^sup>9\<close>), \<^term>\<open>kilo\<close> (\<open>=10\<^sup>3\<close>),  \<^term>\<open>milli\<close> (\<open>=10\<^sup>-\<^sup>3\<close>), etc. 
+\<^vs>\<open>-0.5cm\<close>
 \<close>
 
-
-figure*[induct_type_set::figure, relative_width="85", 
+figure*[induct_type_set::figure, relative_width="60", 
         src="''figures/induct_type_class_scheme.png''"]
 \<open>The "Inductive" Subset of \<open>dim_types\<close>-types interpreted in the \<open>Dimension\<close>-Type\<close>
 
@@ -229,7 +213,7 @@ section*[bgr::background,main_author="Some(@{author ''bu''})"]
 text\<open>This work uses a number of features of Isabelle/HOL and its
 meta-logic Isabelle/Pure, that are not necessarily available in another
 system of the LCF-Prover family and that needs therefore some explanation.
-These concepts are in particular:\<close>
+These concepts are in particular: \<^vs>\<open>-0.3cm\<close>\<close>
 
 subsection\<open>Type-Classes\<close>
 text\<open>
@@ -239,20 +223,21 @@ text\<open>
   and represent therefore a restricted form of dependent types
   (c.f. \<^url>\<open>https://isabelle.in.tum.de/dist/Isabelle2021-1/doc/classes.pdf\<close>). 
   For example, it is possible to define a type-class \<open>preorder\<close> which
-  carries syntactic as well as semantic requirements on  type-instances:
+  carries syntactic as well as semantic requirements on  type-instances: \<^vs>\<open>-0.3cm\<close>
 
 @{theory_text [display, indent=3] \<open>
 class ord =
   fixes less_eq :: "'a \<Rightarrow> 'a \<Rightarrow> bool"
-begin notation  less_eq  ("'(\<le>')")  end
+begin notation  less_eq  ("'(\<le>')")  end\<close>}
 
+@{theory_text [display, indent=3] \<open>
 class preorder = ord +
   assumes order_refl : "x \<le> x"
   and    order_trans : "x \<le> y \<Longrightarrow> y \<le> z \<Longrightarrow> x \<le> z"
 begin ... end
 \<close>}
   
-  An instantiation of this class with the concrete type \<^typ>\<open>nat\<close> has then the format:
+\<^noindent> An instantiation of this class with the concrete type \<^typ>\<open>nat\<close> has then the format:
 
 @{theory_text [display, indent=3] \<open>
 instantiation nat :: preorder
@@ -262,8 +247,8 @@ instance   <instance proof establishing order_refl and order_trans>
 end
 \<close>}
 
-  Note that instantiations are also possible for parametric type constructors such as 
-  \<^typ>\<open>('\<alpha>::preorder) list\<close>: here, an instantiation may use the preorder of the argument
+\<^noindent> Note that instantiations are also possible for parametric type constructors such as 
+  \<^typ>\<open>('\<alpha>::preorder) list\<close>: an instantiation may use the preorder of the argument
   class \<^typ>\<open>'\<alpha>::preorder\<close> both in the definition as well as the proof part.
   Note further, that we will use \<^theory_text>\<open>nat\<close> and \<^typ>\<open>\<nat>\<close> as type synonyms in this paper.
 \<close>
@@ -296,13 +281,28 @@ as the \<^theory_text>\<open>eval\<close>-proof method.
 \<close>
 
 subsection\<open>The lifting package\<close>
-text \<open>
-MORE TO COME
+figure*[lifting::figure, relative_width="40", src="''figures/lifting.png''"]
+\<open>Lifting a binary operation \<open>f\<^sub>C\<close> to \<open>f\<^sub>A\<close>\<close>
+
+
+text \<open>Since type-definitions define new types \<open>\<tau>\<^sub>A\<close> in terms of a subset of values of 
+an implementing (concrete) type \<open>\<tau>\<^sub>C\<close> along the isomorphism represented by functions
+\<open>(Abs,Rep)\<close>, a particular construction called \<^emph>\<open>lifting\<close> is a recurrent scheme 
+for which Isabelle offers support by an own specification construct 
+(see @{cite "HuffmanK13"} for the theoretical foundation). The construction
+has the pattern for the binary case (cf. @{figure \<open>lifting\<close>}): 
+
+@{theory_text [display, indent=3] \<open>lift_definition f\<^sub>A :: "\<tau>\<^sub>A \<times> \<tau>\<^sub>A \<Rightarrow> \<tau>\<^sub>A"  is "f\<^sub>C"\<close>}
+
+\<^noindent> Besides compactness and conciseness, liftings have the advantage to setup 
+the code-generator appropriately, such that calculations on \<open>\<tau>\<^sub>A\<close> can be mapped 
+automatically on \<open>\<tau>\<^sub>C\<close>
 \<close>
 
 
+
 section*[pas::technical,main_author="Some(@{author ''bu''})"] 
-\<open>Preliminary Algebraic Structures\<close>
+\<open>Preliminaries: Basic Algebraic Structures\<close>
 text\<open>At the core, the multiplicative operation on physical dimension
 results in additions of the exponents of base vectors:
 
@@ -327,7 +327,7 @@ class group_mult = inverse + monoid_mult +
 ... 
 class ab_group_mult = comm_monoid_mult + group_mult
 ...
-abbreviation (input) npower :: "'\<alpha>::{power,inverse} \<Rightarrow> nat \<Rightarrow> '\<alpha>"  ("(_\<^sup>-\<^sup>_)" [1000,999] 999) 
+abbreviation(input) npower::"'\<alpha>::{power,inverse} \<Rightarrow> nat \<Rightarrow> '\<alpha>" ("(_\<^sup>-\<^sup>_)"[1000,999]999) 
   where "npower x n \<equiv> inverse (x ^ n)"
 \<close>
 }
@@ -542,7 +542,7 @@ end\<close>}
 Finally, we introduce some syntactic sugar such as \<open>'\<alpha>\<^sup>4\<close> for \<open>'\<alpha> \<cdot> '\<alpha> \<cdot> '\<alpha> \<cdot> '\<alpha>\<close> or 
 \<open>'\<alpha>\<^sup>-\<^sup>4\<close> for \<open>('\<alpha>\<^sup>4)\<^sup>-\<^sup>1\<close>.
 \<close>
-figure*[induct_type_SML_interpreted::figure, relative_width="85", 
+figure*[induct_type_SML_interpreted::figure, relative_width="60", 
         src="''figures/induct_type_class_scheme_ML.png''"]\<open>
   The "Inductive" subset of \<open>dim_types\<close> interpreted in SML Lists\<close>
 text\<open>
@@ -612,8 +612,9 @@ text \<open> We can now define the type of parameterized quantities
 which have a dimension equal to the semantic interpretation of the \<^typ>\<open>'d::dim_type\<close>:
 
 @{theory_text [display, indent=3] \<open>
-typedef (overloaded) ('\<alpha>, 'd::dim_type, 's::unit_system) QuantT ("_[_, _]" [999,0,0] 999) 
-                     = "{x :: ('\<alpha>, 's) Measurement_System. dim x = dim_ty_sem TYPE('d)}"
+typedef (overloaded) ('\<alpha>, 'd::dim_type, 's::unit_system) QuantT 
+                     ("_[_, _]" [999,0,0] 999) 
+                     = "{x :: ('\<alpha>,'s)Measurement_System. dim x = dim_ty_sem TYPE('d)}"
   morphisms fromQ toQ <non-emptyness proof omitted>
 
 setup_lifting type_definition_QuantT
@@ -637,55 +638,43 @@ lift_definition
   is "(*)" by (simp add: dim_ty_sem_DimTimes_def times_Quantity_ext_def)
 
 lift_definition 
-  qinverse :: "('\<alpha>::field)['\<tau>::dim_type, 's::unit_system] \<Rightarrow> '\<alpha>['\<tau>-\<^sup>1, 's]" ("(_\<^sup>-\<^sup>\<one>)" [999] 999) 
+  qinverse :: "('\<alpha>::field)['\<tau>::dim_type,'s::unit_system] \<Rightarrow>'\<alpha>['\<tau>-\<^sup>1,'s]" ("(_\<^sup>-\<^sup>\<one>)"[999]999) 
   is "inverse" by (simp add: inverse_Quantity_ext_def dim_ty_sem_DimInv_def)\<close>}
 
   Additionally, a scalar product \<^term>\<open>(*\<^sub>Q)\<close> and an addition on the magnitude component is 
   introduced that preserves the algebraic properties of the magnitude type:
 
 @{theory_text [display, indent=3] \<open>
-lift_definition scaleQ 
-      :: "'\<alpha> \<Rightarrow> '\<alpha>::comm_ring_1['d::dim_type, 's::unit_system] \<Rightarrow> '\<alpha>['d, 's]" (infixr "*\<^sub>Q" 63)
+lift_definition scaleQ::"'\<alpha>\<Rightarrow>'\<alpha>::comm_ring_1['d::dim_type,'s::unit_system]\<Rightarrow>'\<alpha>['d,'s]"
+                 (infixr"*\<^sub>Q"63)
     is "\<lambda> r x. \<lparr> mag = r * mag x, dim = dim_ty_sem TYPE('d), unit_sys = unit \<rparr>" <proof>
 
 instantiation QuantT :: (plus, dim_type, unit_system) plus
 begin
 lift_definition plus_QuantT :: "'\<alpha>['d, 's] \<Rightarrow> '\<alpha>['d, 's] \<Rightarrow> '\<alpha>['d, 's]"
-  is "\<lambda> x y. \<lparr> mag = mag x + mag y, dim = dim_ty_sem TYPE('d), unit_sys = unit \<rparr>" <proof>
+  is "\<lambda> x y. \<lparr> mag = mag x+mag y, dim = dim_ty_sem TYPE('d),unit_sys = unit \<rparr>" <proof>
 instance ..
 end
-\<close>}
+\<close>}\<close>
 
-
-\<close>
-
-
-(*
-text \<open> Since quantities can have dimension type expressions that are distinct, but denote the same
-  dimension, it is necessary to define the following function for coercion between two dimension
-  expressions. This requires that the underlying dimensions are the same. 
-
-@{theory_text [display, indent=3] \<open>
-definition coerceQuantT :: 
-           "'d\<^sub>2 itself \<Rightarrow> '\<alpha>['d\<^sub>1::dim_type, 's::unit_system] \<Rightarrow> '\<alpha>['d\<^sub>2::dim_type, 's]" 
-  where [si_def]: "dim_ty_sem TYPE('d\<^sub>1) = dim_ty_sem TYPE('d\<^sub>1) 
-                   \<Longrightarrow> coerceQuantT t x = (toQ (fromQ x))" \<close>}
-and add additional syntax that allows for abbreviating \<open>coerceQuantT TYPE('\<tau>)\<close> by \<open>QCOERCE[\<tau>]\<close>
-\<close>
-*)
 subsection \<open> Predicates on Typed Quantities \<close>
 
 text \<open> The standard HOL order \<^term>\<open>(\<le>)\<close> and equality \<^term>\<open>(=)\<close> have the homogeneous type
   \<^typ>\<open>'a \<Rightarrow> 'a \<Rightarrow> bool\<close> and so they cannot compare values of different types. Consequently,
   we define a heterogeneous order and equivalence on typed quantities. 
-  Both operations were defined as lifting of the core operations.
+  Both operations were defined as lifting of the core operations, and exploit 
+  the semantic interpretation of \<^typ>\<open>'d::dim_type\<close> as shown in 
+  @{figure \<open>induct_type_set\<close>} and were constructed as liftings over the equality 
+  and order on \<^typ>\<open>Dimension\<close>'s.
 
 @{theory_text [display, indent=3] \<open>
-lift_definition qless_eq :: "'\<alpha>::order['d::dim_type,'s::unit_system] \<Rightarrow> '\<alpha>['d::dim_type,'s] \<Rightarrow> bool" 
-  (infix "\<lesssim>\<^sub>Q" 50) is "(\<le>)" .
+lift_definition qless_eq :: 
+                "'\<alpha>::order['d::dim_type,'s::unit_system] \<Rightarrow> '\<alpha>['d::dim_type,'s] \<Rightarrow> bool"
+                (infix "\<lesssim>\<^sub>Q" 50) is "(\<le>)" .
 
-lift_definition qequiv :: "'\<alpha>['d\<^sub>1::dim_type, 's::unit_system] \<Rightarrow> '\<alpha>['d\<^sub>2::dim_type, 's] \<Rightarrow> bool" 
-  (infix "\<cong>\<^sub>Q" 50) is "(=)" .
+lift_definition qequiv :: 
+                "'\<alpha>['d\<^sub>1::dim_type, 's::unit_system] \<Rightarrow> '\<alpha>['d\<^sub>2::dim_type, 's] \<Rightarrow> bool" 
+                (infix "\<cong>\<^sub>Q" 50) is "(=)" .
 \<close>}
 
   These are both fundamentally the same as the usual order and equality relations, but they
@@ -707,1009 +696,73 @@ or the US-customer system (UCS). If needed, type-safe conversion operations betw
 systems can be defined, whose precision will depend on the underlying magnitude types, however.  
 \<close>
 
+subsection \<open> SI Prefixes \<close>
+text \<open>The VIM defines in its SI part aa number of prefixes are simply numbers 
+that can be composed with units using the scalar multiplication operator
+\<^term>\<open>(*\<^sub>Q)\<close>. These are in particular:
+
+@{theory_text [display, indent=3] \<open>
+
+definition deca :: "'a" where [si_eq]: "deca = 10^1"
+definition hecto :: "'a" where [si_eq]: "hecto = 10^2"
+definition kilo :: "'a" where [si_eq]: "kilo = 10^3"
+definition mega :: "'a" where [si_eq]: "mega = 10^6"
+
+...
+
+definition deci :: "'a" where [si_eq]: "deci = 1/10^1"
+definition centi :: "'a" where [si_eq]: "centi = 1/10^2"
+definition milli :: "'a" where [si_eq]: "milli = 1/10^3"
+definition micro :: "'a" where [si_eq]: "micro = 1/10^6"
+...
+\<close>}
+
+
+For example, it is therefore possible to represent 
+and prove the following scalar calculations:
+
+@{theory_text [display, indent=3] \<open>
+lemma "2.3 *\<^sub>Q (centi *\<^sub>Q metre)\<^sup>\<three> = 2.3 \<cdot> 1/10^6 *\<^sub>Q metre\<^sup>\<three>"
+  by (si_simp)
+
+lemma "1 *\<^sub>Q (centi *\<^sub>Q metre)\<^sup>-\<^sup>\<one> = 100 *\<^sub>Q metre\<^sup>-\<^sup>\<one>"
+  by (si_simp)
+\<close>}
+\<close>
+
+
 section*[expls::example,main_author="Some(@{author ''bu''})"] 
 \<open>Validation by the VIM and the 'Brochure'\<close>
 
 section\<open>Related Work and Conclusion\<close>
+text\<open>
+For example, the crucial definitions adapted from the SI Brochure that 
+give the concrete definitions for the metre and the kilogram can be presented as follows: \<^vs>\<open>0.3cm\<close>
+
+\<^theory_text>\<open>theorem metre_definition\<close>
+\<^item> @{term [show_types=false]\<open>1 *\<^sub>Q metre \<cong>\<^sub>Q \<^bold>c \<^bold>\<cdot> (299792458 *\<^sub>Q \<one>)\<^sup>-\<^sup>\<one> \<^bold>\<cdot> second\<close>}
+\<^item> @{term [show_types=false]\<open>1 *\<^sub>Q metre \<cong>\<^sub>Q 9192631770 / 299792458 *\<^sub>Q \<^bold>c \<^bold>\<cdot> (9192631770 *\<^sub>Q second\<^sup>-\<^sup>\<one>)\<^sup>-\<^sup>\<one>\<close>}
+
+\<^noindent> \<^theory_text>\<open>theorem kilogram_definition\<close>
+\<^item> \<^term>\<open>((1 *\<^sub>Q kilogram)::('\<alpha>::field_char_0) kilogram) \<cong>\<^sub>Q (\<^bold>h \<^bold>/ (6.62607015 \<cdot> 1/(10^34) *\<^sub>Q \<one>))\<^bold>\<cdot>metre\<^sup>-\<^sup>\<two>\<^bold>\<cdot>second\<close> 
+\<close>
+
+text\<open>
+These equations give the concrete definitions for the 
+metre and kilogram in terms of the physical constants \<^term>\<open>\<^bold>c\<close> (speed of light) and \<^term>\<open>\<^bold>h\<close> 
+(Planck constant). They can be proven directly using the tactic \<^theory_text>\<open>si-calc\<close> provided by our theory.
+\<close>
+
 text\<open>
 
 This work has drawn inspiration from some previous formalisations of the ISQ and SI, notably Hayes 
 and Mahoney's formalisation in Z@{cite "HayesBrendan95"} and Aragon's algebraic structure for physical
 quantities@{cite "Aragon2004-SI"}. To the best of our knowledge, our mechanisation represents the 
 most comprehensive account of ISQ and SI in a theory prover.
+
+\pagebreak
 \<close>
 
-text\<open>\pagebreak\<close>
-
-(*<*)
-section\<open>Annex\<close>
-
-subsection\<open>Alien stuff - Examples to Typeset in DOF.\<close>
-
-text\<open>
-
-Communicating Sequential Processes (\<^csp>) is a language 
-to specify and verify patterns of interaction of concurrent systems.
-Together with CCS and LOTOS, it belongs to the family of \<^emph>\<open>process algebras\<close>. 
-\<^csp>'s rich theory comprises denotational, operational and algebraic semantic facets 
-and has influenced programming languages such as Limbo, Crystal, Clojure and
-most notably Golang @{cite "donovan2015go"}. \<^csp> has been applied in 
-industry as a tool for specifying and verifying the concurrent aspects of hardware 
-systems, such as the T9000 transansputer @{cite "Barret95"}. 
-
-The theory of \<^csp> was first described in 1978 in a book by Tony Hoare @{cite "Hoare:1985:CSP:3921"}, 
-but has since evolved substantially @{cite "BrookesHR84" and "brookes-roscoe85" and "roscoe:csp:1998"}.
-\<^csp> describes the most common communication and synchronization mechanisms
-with one single language primitive: synchronous communication written \<open>_\<lbrakk>_\<rbrakk>_\<close>. \<^csp> semantics is 
-described by a fully abstract model of behaviour designed to be \<^emph>\<open>compositional\<close>: the denotational
-semantics of a possible environments \<open>P \<lbrakk>S\<rbrakk> Env\<close> (where \<open>S\<close> is the set of \<open>atomic events\<close> both \<open>P\<close> and \<open>Env\<close> must
-synchronize). This design objective has the consequence that two kinds of choice have to 
-be distinguished: 
-  \<^enum> the \<^emph>\<open>external choice\<close>, written \<open>_\<box>_\<close>, which forces a process "to follow" whatever
-    the environment offers, and
-  \<^enum> the \<^emph>\<open>internal choice\<close>, written \<open>_\<sqinter>_\<close>, which imposes on the environment of a process 
-    "to follow" the non-deterministic choices made.
-
-\<close>
-
-(*>*)
-(*
-text\<open>
-Generalizations of these two operators \<open>\<box>x\<in>A. P(x)\<close> and \<open>\<Sqinter>x\<in>A. P(x)\<close> allow for modeling the concepts 
-of \<^emph>\<open>input\<close> and \<^emph>\<open>output\<close>: Based on the prefix operator \<open>a\<rightarrow>P\<close> (event \<open>a\<close> happens, then the process 
-proceeds with \<open>P\<close>), receiving input is modeled by \<open>\<box>x\<in>A. x\<rightarrow>P(x)\<close> while sending output is represented 
-by \<open>\<Sqinter>x\<in>A. x\<rightarrow>P(x)\<close>. Setting choice in the center of the language semantics implies that 
-deadlock-freeness becomes a vital property for the well-formedness of a process, nearly as vital
-as type-checking: Consider two events \<open>a\<close> and \<open>b\<close> not involved in a process \<open>P\<close>, then
-\<open>(a\<rightarrow>P \<box> b\<rightarrow>P) \<lbrakk>{a,b}\<rbrakk> (a\<rightarrow>P \<sqinter> b\<rightarrow>P)\<close> is deadlock free provided \<open>P\<close> is, while
-\<open>(a\<rightarrow>P \<sqinter> b\<rightarrow>P) \<lbrakk>{a,b}\<rbrakk> (a\<rightarrow>P \<sqinter> b\<rightarrow>P)\<close> deadlocks (both processes can make "ruthlessly" an opposite choice,
-but are required to synchronize). 
-
-Verification of \<^csp> properties has been centered around the notion of \<^emph>\<open>process refinement orderings\<close>,
-most notably \<open>_\<sqsubseteq>\<^sub>F\<^sub>D_\<close> and \<open>_\<sqsubseteq>_\<close>. The latter turns the denotational domain of \<^csp> into a Scott cpo 
-@{cite "scott:cpo:1972"}, which yields semantics for the fixed point operator \<open>\<mu>x. f(x)\<close> provided 
-that \<open>f\<close> is continuous with respect to \<open>_\<sqsubseteq>_\<close>. Since it is possible to express deadlock-freeness and 
-livelock-freeness as a refinement problem, the verification of properties has been reduced 
-traditionally to a model-checking problem for finite set of events \<open>A\<close>.
-
-We are interested in verification techniques for arbitrary event sets \<open>A\<close> or arbitrarily 
-parameterized processes. Such processes can be used to model dense-timed processes, processes 
-with dynamic thread creation, and processes with unbounded thread-local variables and buffers. 
-However, this adds substantial complexity to the process theory: when it comes to study the 
-interplay of different denotational models, refinement-orderings, and side-conditions for 
-continuity, paper-and-pencil proofs easily reach their limits of precision. 
-
-Several attempts have been undertaken to develop a formal theory in an interactive proof system, 
-mostly in Isabelle/HOL @{cite "Camilleri91" and "tej.ea:corrected:1997" and  "IsobeRoggenbach2010"
-and "DBLP:journals/afp/Noce16"}.
-This paper is based on @{cite "tej.ea:corrected:1997"}, which has been the most comprehensive 
-attempt to formalize denotational \<^csp> semantics covering a part of Bill Roscoe's Book 
-@{cite "roscoe:csp:1998"}. Our contributions are as follows:
-  \<^item>  we ported @{cite "tej.ea:corrected:1997"} from Isabelle93-7 and ancient 
-    ML-written proof scripts to a modern Isabelle/HOL version and structured Isar proofs,
-    and extended it substantially,
-  \<^item> we introduced new refinement notions allowing a deeper understanding of the \<^csp>
-    Failure/Divergence model, providing some meta-theoretic clarifications,
-  \<^item> we used our framework to derive new types of decomposition rules  and 
-    stronger induction principles based on the new refinement notions, and
-  \<^item> we integrate this machinery into a number of advanced verification techniques, which we 
-    apply to two generalized paradigmatic examples in the \<^csp> literature,
-    the CopyBuffer and Dining Philosophers@{footnote \<open>All proofs concerning the 
-    HOL-CSP 2 core have been published in the Archive of  Formal Proofs @{cite "HOL-CSP-AFP"}; 
-    all other proofs are available at 
-    \<^url>\<open>https://gitlri.lri.fr/burkhart.wolff/hol-csp2.0\<close>. In this paper, all Isabelle proofs are 
-    omitted.\<close>}. 
-\<close>
-
-
-(*
-% Moreover, decomposition rules of the form:
-% \begin{center}
-% \begin{minipage}[c]{10cm}
-%    @{cartouche [display] \<open>C \<Longrightarrow> A \<sqsubseteq>\<^sub>F\<^sub>D A' \<Longrightarrow> B \<sqsubseteq>\<^sub>F\<^sub>D B' \<Longrightarrow> A \<lbrakk>S\<rbrakk> B \<sqsubseteq>\<^sub>F\<^sub>D A' \<lbrakk>S\<rbrakk> B'\<close>}
-% \end{minipage}
-% \end{center} 
-% are of particular interest since they allow to avoid the costly automata-product construction 
-% of model-checkers and to separate infinite sub-systems from finite (model-checkable) ones; however,
-% their side-conditions \<open>C\<close> are particularly tricky to work out. Decomposition rules  may pave the 
-% way for future tool combinations for model-checkers such as FDR4~@{cite "fdr4"} or 
-% PAT~@{cite "SunLDP09"} based on proof certifications.*)
-
-
-
-section*["pre"::tc,main_author="Some(@{docitem \<open>bu\<close>}::author)"]
-\<open>Preliminaries\<close>
-
-text\<open>\<close>
-
-subsection*[cspsemantics::tc, main_author="Some(@{docitem ''bu''})"]\<open>Denotational \<^csp> Semantics\<close>
-
-text\<open> The denotational semantics (following @{cite "roscoe:csp:1998"}) comes in three layers: 
-the \<^emph>\<open>trace model\<close>, the \<^emph>\<open>(stable) failures model\<close> and the \<^emph>\<open>failure/divergence model\<close>.
-
-In the trace semantics model, a process \<open>P\<close> is denoted by a set of communication traces,
-built from atomic events. A trace here represents a partial history of the communication 
-sequence occurring when a process interacts with its environment. For the two basic \<^csp> 
-processes \<open>Skip\<close> (successful termination) and \<open>Stop\<close> (just deadlock), the semantic function
-\<open>\<T>\<close> of the trace model just gives the same denotation, \<^ie> the empty trace: 
-\<open>\<T>(Skip) = \<T>(Stop) = {[]}\<close>.
-Note that the trace sets, representing all \<^emph>\<open>partial\<close> history, is in general prefix closed.\<close>
-
-text*[ex1::math_example, status=semiformal] \<open>
-Let two processes be defined as follows:
-
-  \<^enum>  \<open>P\<^sub>d\<^sub>e\<^sub>t = (a \<rightarrow> Stop) \<box> (b \<rightarrow> Stop)\<close>
-  \<^enum> \<open>P\<^sub>n\<^sub>d\<^sub>e\<^sub>t = (a \<rightarrow> Stop) \<sqinter> (b \<rightarrow> Stop)\<close> 
-\<close> 
-
-text\<open>These two processes \<open>P\<^sub>d\<^sub>e\<^sub>t\<close> and \<open>P\<^sub>n\<^sub>d\<^sub>e\<^sub>t\<close> cannot be distinguished by using 
-the trace semantics: \<open>\<T>(P\<^sub>d\<^sub>e\<^sub>t) = \<T>(P\<^sub>n\<^sub>d\<^sub>e\<^sub>t) = {[],[a],[b]}\<close>. To resolve this problem, Brookes @{cite "BrookesHR84"} 
-proposed the failures model, where communication traces were augmented with the 
-constraint information for further communication that is represented negatively as a refusal set. 
-A failure \<open>(t, X)\<close> is a pair of a trace \<open>t\<close> and a set of events \<open>X\<close> that a process can refuse if 
-any of the events in \<open>X\<close> were offered to him by the environment after performing the trace \<open>t\<close>. 
-The semantic function \<open>\<F>\<close> in the failures model maps a process to a set of refusals.
-Let \<open>\<Sigma>\<close> be the set of events. Then, \<open>{([],\<Sigma>)} \<subseteq> \<F> Stop\<close> as the process \<open>Stop\<close> refuses all events. 
-For Example 1, we have \<open>{([],\<Sigma>\{a,b}),([a],\<Sigma>),([b],\<Sigma>)} \<subseteq> \<F> P\<^sub>d\<^sub>e\<^sub>t\<close>, while
-\<open>{([],\<Sigma>\{a}),([],\<Sigma>\{b}),([a],\<Sigma>),([b],\<Sigma>)} \<subseteq> \<F> P\<^sub>n\<^sub>d\<^sub>e\<^sub>t\<close> (the \<open>_\<subseteq>_\<close> refers to the fact that
-the refusals must be downward closed; we show only the maximal refusal sets here).
-Thus, internal and external choice, also called \<^emph>\<open>nondeterministic\<close> and \<^emph>\<open>deterministic\<close>
-choice, can be distinguished in the failures semantics.
-
-However, it turns out that the failures model suffers from another deficiency with respect to 
-the phenomenon called infinite internal chatter or \<^emph>\<open>divergence\<close>.\<close>
-
-text*[ex2::example, status=semiformal] \<open>
-The following process \<open>P\<^sub>i\<^sub>n\<^sub>f\<close> is an infinite process that performs \<open>a\<close> infinitely 
-many times. However, using the \<^csp> hiding operator \<open>_\_\<close>, this activity is concealed: 
-
-  \<^enum>  \<open>P\<^sub>i\<^sub>n\<^sub>f = (\<mu> X. a \<rightarrow> X) \ {a}\<close>
-
-\<close>
-
-text\<open>where \<open>P\<^sub>i\<^sub>n\<^sub>f\<close> will be equivalent to \<open>\<bottom>\<close> in the process cpo ordering. 
-To distinguish divergences from the deadlock process, Brookes and Roscoe 
-proposed failure/divergence model to incorporate divergence traces  @{cite "brookes-roscoe85"}. 
-A divergence trace is the one leading to a possible divergent behavior. 
-A well behaved process should be able to respond to its environment in a finite amount of time. 
-Hence, divergences are considered as a kind of a catastrophe in this model. 
-Thus, a process is represented by a failure set \<open>\<F>\<close>, 
-together with a set of divergence traces \<open>\<D>\<close>;
-in our example, the empty trace \<open>[]\<close> belongs to \<open>\<D> P\<^sub>i\<^sub>n\<^sub>f\<close>.
-
-The failure/divergence model has become the standard semantics for an enormous range of \<^csp> 
-research and the implementations of @{cite "fdr4" and "SunLDP09"}. Note, that the work
-of @{cite "IsobeRoggenbach2010"} is restricted to a variant of the failures model only.
- 
-\<close>
-
-subsection*["isabelleHol"::tc, main_author="Some(@{docitem ''bu''})"]\<open>Isabelle/HOL\<close>
-text\<open> Nowadays, Isabelle/HOL is one of the major interactive theory development environments
-@{cite "nipkow.ea:isabelle:2002"}. HOL stands for Higher-Order Logic, a logic based on simply-typed
-\<open>\<lambda>\<close>-calculus extended by parametric polymorphism and Haskell-like type-classes.
-Besides interactive and integrated automated proof procedures,
-it offers code and documentation generators. Its structured proof language Isar is intensively used
-in the plethora of work done and has been a key factor for the success of the Archive of Formal Proofs
-(\<^url>\<open>https://www.isa-afp.org\<close>).
-
-For the work presented here, one relevant construction is :
-
-   \<^item> \<^theory_text>\<open>typedef  (\<alpha>\<^sub>1,...,\<alpha>\<^sub>n)t = E\<close>
-
- 
-It creates a fresh type that is isomorphic to a set \<open>E\<close> involving \<open>\<alpha>\<^sub>1,...,\<alpha>\<^sub>n\<close> types.
-Isabelle/HOL performs a number of syntactic checks for these constructions that guarantee the logical
-consistency of the defined constants or types relative to the axiomatic basis of HOL. The system
-distribution comes with rich libraries comprising Sets, Numbers, Lists, etc. which are built in this
-"conservative" way.
-
-For this work, a particular library called \<^theory_text>\<open>HOLCF\<close> is intensively used. It provides classical 
-domain theory for a particular type-class \<open>\<alpha>::pcpo\<close>, \<^ie> the class of types  \<open>\<alpha>\<close> for which 
-
-   \<^enum>  a least element \<open>\<bottom>\<close> is defined, and
-   \<^enum> a complete partial order \<open>_\<sqsubseteq>_\<close> is defined.
-
- For these types, \<^theory_text>\<open>HOLCF\<close> provides a fixed-point operator \<open>\<mu>X. f X\<close> as well as the 
-fixed-point induction and other (automated) proof infrastructure. Isabelle's type-inference can 
-automatically infer, for example, that if \<open>\<alpha>::pcpo\<close>, then \<open>(\<beta> \<Rightarrow> \<alpha>)::pcpo\<close>. \<close>
-  
-section*["csphol"::tc,main_author="Some(@{docitem ''bu''}::author)", level="Some 2"]
-\<open>Formalising Denotational \<^csp> Semantics in HOL \<close>
-
-text\<open>\<close>
-
-subsection*["processinv"::tc, main_author="Some(@{docitem ''bu''})"]
-\<open>Process Invariant and Process Type\<close>
-text\<open> First, we need a slight revision of the concept
-of \<^emph>\<open>trace\<close>: if \<open>\<Sigma>\<close> is the type of the atomic events (represented by a type variable), then
-we need to extend this type by a special event \<open>\<surd>\<close> (called "tick") signaling termination.
-Thus, traces have the type \<open>(\<Sigma>+\<surd>)\<^sup>*\<close>, written \<open>\<Sigma>\<^sup>\<surd>\<^sup>*\<close>; since \<open>\<surd>\<close> may only occur at the end of a trace, 
-we need to define a predicate \<open>front\<^sub>-tickFree t\<close> that requires from traces that \<open>\<surd>\<close> can only occur 
-at the end.
-
-Second, in the traditional literature, the semantic domain is implicitly described by 9 "axioms" 
-over the three semantic functions \<open>\<T>\<close>, \<open>\<F>\<close> and \<open>\<D>\<close>.
-Informally, these are:
-
-   \<^item> the initial trace of a process must be empty;
-   \<^item> any allowed trace must be \<open>front\<^sub>-tickFree\<close>; 
-   \<^item> traces of a process are  \<^emph>\<open>prefix-closed\<close>; 
-   \<^item> a process can refuse all subsets of a refusal set; 
-   \<^item> any event refused by a process after a trace \<open>s\<close> must be in a refusal set associated to \<open>s\<close>;
-   \<^item> the tick accepted after a trace \<open>s\<close> implies that all other events are refused; 
-   \<^item> a divergence trace with any suffix is itself a divergence one
-   \<^item> once a process has diverged, it can engage in or refuse any sequence of events.
-   \<^item> a trace ending with \<open>\<surd>\<close> belonging to divergence set implies that its 
-     maximum prefix without \<open>\<surd>\<close> is also a divergent trace.
-
-More formally, a process \<open>P\<close> of the type \<open>\<Sigma> process\<close> should have the following properties:
-
-
-@{cartouche [display] \<open>([],{}) \<in> \<F> P \<and>
-(\<forall> s X.  (s,X) \<in> \<F> P \<longrightarrow> front_tickFree s) \<and>
-(\<forall> s t . (s@t,{}) \<in> \<F> P \<longrightarrow> (s,{}) \<in> \<F> P) \<and>
-(\<forall> s X Y. (s,Y) \<in> \<F> P \<and> X\<subseteq>Y \<longrightarrow> (s,X) \<in> \<F> P) \<and> 
-(\<forall> s X Y. (s,X) \<in> \<F> P \<and> (\<forall>c \<in> Y. ((s@[c],{}) \<notin> \<F> P)) \<longrightarrow> (s,X \<union> Y) \<in> \<F> P) \<and>
-(\<forall> s X.  (s@[\<surd>],{}) \<in> \<F> P \<longrightarrow> (s,X-{\<surd>}) \<in> \<F> P) \<and>
-(\<forall> s t. s \<in> \<D> P \<and> tickFree s \<and> front_tickFree t \<longrightarrow> s@t \<in> \<D> P)  \<and>
-(\<forall> s X. s \<in> \<D> P \<longrightarrow> (s,X) \<in> \<F> P) \<and>
-(\<forall> s. s@[\<surd>] \<in> \<D> P \<longrightarrow> s \<in> \<D> P)\<close>}
-
-Our objective is to encapsulate this wishlist into a type constructed as a conservative
-theory extension in our theory \<^holcsp>.
-Therefore third, we define a pre-type for processes \<open>\<Sigma> process\<^sub>0\<close> by \<open> \<P>(\<Sigma>\<^sup>\<surd>\<^sup>* \<times> \<P>(\<Sigma>\<^sup>\<surd>)) \<times> \<P>(\<Sigma>\<^sup>\<surd>)\<close>.
-Forth, we turn our wishlist of "axioms" above into the definition of a predicate \<open>is_process P\<close> 
-of type \<open>\<Sigma> process\<^sub>0 \<Rightarrow> bool\<close> deciding if its conditions are fulfilled. Since \<open>P\<close> is a pre-process,
-we replace \<open>\<F>\<close> by \<open>fst\<close> and  \<open>\<D>\<close> by \<open>snd\<close> (the HOL projections into a pair).
-And last not least fifth, we use the following type definition:
-  \<^item> \<^theory_text>\<open>typedef '\<alpha> process = "{P :: '\<alpha> process\<^sub>0 . is_process P}"\<close>
-
-
-Isabelle requires a proof for the existence of a witness for this set,
-but this can be constructed in a straight-forward manner. Suitable definitions for 
-\<open>\<T>\<close>, \<open>\<F>\<close> and \<open>\<D>\<close> lifting \<open>fst\<close> and \<open>snd\<close> on the new \<open>'\<alpha> process\<close>-type allows to derive
-the above properties for any \<open>P::'\<alpha> process\<close>. \<close>
-
-subsection*["operator"::tc, main_author="Some(@{docitem ''lina''})"]
-\<open>\<^csp> Operators over the Process Type\<close>
-text\<open> Now, the operators of \<^csp> \<open>Skip\<close>, \<open>Stop\<close>, \<open>_\<sqinter>_\<close>,  \<open>_\<box>_\<close>, \<open>_\<rightarrow>_\<close>,\<open>_\<lbrakk>_\<rbrakk>_\<close> etc. 
-for internal choice, external choice, prefix and parallel composition, can 
-be defined indirectly on the process-type. For example, for the simple case of the internal choice,
-we construct it such that \<open>_\<sqinter>_\<close> has type \<open>'\<alpha> process \<Rightarrow> '\<alpha> process \<Rightarrow> '\<alpha> process\<close> and 
-such that its projection laws satisfy the properties \<open>\<F> (P \<sqinter> Q) = \<F> P \<union> \<F> Q\<close>  and 
-\<open>\<D> (P \<sqinter> Q) = \<D> P \<union> \<D> Q\<close> required from @{cite "roscoe:csp:1998"}. 
-This boils down to a proof that an equivalent definition on the pre-process type \<open>\<Sigma> process\<^sub>0\<close>
-maintains \<open>is_process\<close>, \<^ie> this predicate remains invariant on the elements of the semantic domain. 
-For example, we define \<open>_\<sqinter>_\<close> on the pre-process type as follows:
-
-  \<^item> \<^theory_text>\<open>definition "P \<sqinter> Q \<equiv> Abs_process(\<F> P \<union> \<F> Q , \<D> P \<union> \<D> Q)"\<close>
-
-where \<open>\<F> = fst \<circ> Rep_process\<close> and \<open>\<D> = snd \<circ> Rep_process\<close> and where \<open>Rep_process\<close> and
-\<open>Abs_process\<close> are the representation and abstraction morphisms resulting from the
-type definition linking \<open>'\<alpha> process\<close> isomorphically to \<open>'\<alpha> process\<^sub>0\<close>. Proving the above properties
-for  \<open>\<F> (P \<sqinter> Q)\<close> and \<open>\<D> (P \<sqinter> Q)\<close> requires a proof that \<open>(\<F> P \<union> \<F> Q , \<D> P \<union> \<D> Q)\<close>
-satisfies the 9 "axioms", which is fairly simple in this case.
-
-The definitional presentation of the \<^csp> process operators according to @{cite "roscoe:csp:1998"} 
-follows always this scheme. This part of the theory comprises around 2000 loc. 
-\<close>
-
-subsection*["orderings"::tc, main_author="Some(@{docitem ''bu''})"]
-\<open>Refinement Orderings\<close>
-
-text\<open> \<^csp> is centered around the idea of process refinement; many critical properties, 
-even ones typically considered as "liveness-properties", can be expressed in terms of these, and
-a conversion of processes in terms of (finite) labelled transition systems leads to effective
-model-checking techniques based on graph-exploration. Essentially,  a process \<open>P\<close> \<^emph>\<open>refines\<close> 
-another process \<open>Q\<close> if and only if it is more deterministic and more defined (has less divergences).
-Consequently, each of the three semantics models (trace, failure and failure/divergence) 
-has its corresponding refinement orderings. 
-What we are interested in this paper is the following refinement orderings for the 
-failure/divergence model.
-
-   \<^enum> \<open>P \<sqsubseteq>\<^sub>\<F>\<^sub>\<D> Q \<equiv> \<F> P \<supseteq> \<F> Q \<and> \<D> P \<supseteq> \<D> Q\<close> 
-   \<^enum> \<open>P \<sqsubseteq>\<^sub>\<T>\<^sub>\<D> Q \<equiv> \<T> P \<supseteq> \<T> Q \<and> \<D> P \<supseteq> \<D> Q\<close>
-   \<^enum> \<open>P \<sqsubseteq>\<^sub>\<FF> Q \<equiv>  \<FF> P \<supseteq> \<FF> Q, \<FF>\<in>{\<T>,\<F>,\<D>}\<close> 
-
- Notice that in the \<^csp> literature, only \<open>\<sqsubseteq>\<^sub>\<F>\<^sub>\<D>\<close> is well studied for failure/divergence model. 
-Our formal analysis of different granularities on the refinement orderings   
-allows deeper understanding of the same semantics model. For example, \<open>\<sqsubseteq>\<^sub>\<T>\<^sub>\<D>\<close> turns
-out to have in some cases better monotonicity properties and therefore allow for stronger proof
-principles in \<^csp>. Furthermore, the refinement ordering \<open>\<sqsubseteq>\<^sub>\<F>\<close> analyzed here 
-is different from the classical 
-failure refinement in the literature that is studied for the stable failure model  
-@{cite "roscoe:csp:1998"}, where failures are only defined for stable 
-states, from which no internal progress is possible. 
-\<close>
-
-
-subsection*["fixpoint"::tc, main_author="Some(@{docitem ''lina''})"]
-\<open>Process Ordering and HOLCF\<close>
-text\<open> For any denotational semantics, the fixed point theory giving semantics to systems
-of recursive equations is considered as keystone. Its prerequisite is a complete partial ordering
-\<open>_\<sqsubseteq>_\<close>. The natural candidate \<open>_\<sqsubseteq>\<^sub>\<F>\<^sub>\<D>_\<close> is unfortunately not complete for infinite \<open>\<Sigma>\<close> for the
-generalized deterministic choice, and thus for the building block of the read-operations.
-
-Roscoe and Brooks @{cite "Roscoe1992AnAO"} finally proposed another ordering, called the 
-\<^emph>\<open>process ordering\<close>, and restricted the generalized deterministic choice in a particular way such 
-that completeness could at least be assured for read-operations. This more complex ordering 
-is based on the concept \<^emph>\<open>refusals after\<close> a trace \<open>s\<close> and defined by \<open>\<R> P s \<equiv> {X | (s, X) \<in> \<F> P}\<close>.\<close>
-
-Definition*[process_ordering, short_name="''process ordering''"]\<open>
-We define \<open>P \<sqsubseteq> Q \<equiv> \<psi>\<^sub>\<D> \<and> \<psi>\<^sub>\<R> \<and> \<psi>\<^sub>\<M> \<close>,  where 
-\<^enum>  \<open>\<psi>\<^sub>\<D> = \<D> P \<supseteq> \<D> Q \<close>
-\<^enum> \<open>\<psi>\<^sub>\<R> = s \<notin> \<D> P \<Rightarrow> \<R> P s = \<R> Q s\<close>  
-\<^enum> \<open>\<psi>\<^sub>\<M> = Mins(\<D> P) \<subseteq> \<T> Q \<close> 
-\<close>
-
-text\<open>The third condition \<open>\<psi>\<^sub>\<M>\<close> implies that the set of minimal divergent traces 
-(ones with no proper prefix that is also a divergence) in  \<open>P\<close>,  denoted by \<open>Mins(\<D> P)\<close>, 
-should be a subset of the trace set of \<open>Q\<close>. 
-%One may note that each element in \<open>Mins(\<D> P)\<close> do actually not contain the \<open>\<surd>\<close>, 
-%which can be deduced from the process invariants described 
-%in the precedent @{technical "processinv"}. This can be explained by the fact that we are not 
-%really concerned with what a process does after it terminates. 
-It is straight-forward to define the least element \<open>\<bottom>\<close> in this ordering by 
-\<open>\<F>(\<bottom>)= {(s,X). front_tickFree s}\<close> and  \<open>\<D>(\<bottom>) = {s. front_tickFree s}\<close>  \<close>
-
-text\<open>While the original work @{cite "tej.ea:corrected:1997"} was based on an own --- and different ---
-fixed-point theory, we decided to base HOL-\<^csp> 2 on HOLCF (initiated by @{cite "muller.ea:holcf:1999"} 
-and substantially extended in @{cite "huffman.ea:axiomatic:2005"}). 
-HOLCF is based on parametric polymorphism with type classes. A type class is actually a 
-constraint on a type variable by respecting certain syntactic and semantics 
-requirements. For example, a type class of partial ordering, denoted by \<open>\<alpha>::po\<close>, is restricted to
-all types \<open>\<alpha>\<close> possessing a relation \<open>\<le>:\<alpha>\<times>\<alpha>\<rightarrow>bool\<close> that is reflexive, anti-symmetric, and transitive.
-Isabelle possesses a construct that allows to establish, that the type \<open>nat\<close> belongs to this class,
-with the consequence that all lemmas derived abstractly on \<open>\<alpha>::po\<close> are in particular applicable on 
-\<open>nat\<close>. The type class of \<open>po\<close> can be extended to the class of complete partial ordering  \<open>cpo\<close>. 
-A \<open>po\<close> is said to be complete if all non-empty directed sets have a least upper bound (\<open>lub\<close>). 
-Finally the class of \<open>pcpo\<close> (Pointed cpo) is a \<open>cpo\<close> ordering that has a least element, 
-denoted by \<open>\<bottom>\<close>. For \<open>pcpo\<close> ordering, two crucial notions for continuity (\<open>cont\<close>) and fixed-point operator 
-(\<open>\<mu>X. f(X)\<close>) are defined in the usual way. A function from one  \<open>cpo\<close> to another one is said 
-to be continuous if it distributes over the \<open>lub\<close> of all directed sets (or chains).
-One key result of the fixed-point theory is the proof of the fixed-point theorem:
-
-@{cartouche [display, indent=25] \<open>cont f \<Longrightarrow>  \<mu>X. f(X) = f(\<mu>X. f(X))\<close>}
-
-For most \<^csp> operators \<open>\<otimes>\<close> we derived rules of the form: 
-   @{cartouche [display, indent=20] \<open>cont P \<Longrightarrow> cont Q \<Longrightarrow> cont(\<lambda>x. (P x) \<otimes> (Q x))\<close>}
-
-These rules allow to automatically infer for any process term if it is continuous or not.  
-The port of HOL-CSP 2 on HOLCF implied that the derivation of the entire continuity rules 
-had to be completely re-done (3000 loc).
-
- 
-HOL-CSP provides an important proof principle, the fixed-point induction:
-
-@{cartouche [display, indent=5] \<open>cont f \<Longrightarrow> adm P \<Longrightarrow> P \<bottom> \<Longrightarrow> (\<And>X. P X \<Longrightarrow> P(f X)) \<Longrightarrow> P(\<mu>X. f X)\<close>}
-
-Fixed-point induction requires a small side-calculus for establishing the admissibility
-of a predicate; basically, predicates are admissible if they are valid for any least upper bound 
-of a chain \<open>x\<^sub>1 \<sqsubseteq> x\<^sub>2 \<sqsubseteq> x\<^sub>3 ... \<close> provided that \<open>\<forall>i. P(x\<^sub>i)\<close>. It turns out that \<open>_\<sqsubseteq>_\<close> and \<open>_\<sqsubseteq>\<^sub>F\<^sub>D_\<close> as
-well as all other refinement orderings that we introduce in this paper are  admissible.
-Fixed-point inductions are the main proof weapon in verifications, 
-together with monotonicities and the \<^csp> laws. Denotational arguments can be hidden as they are not 
-needed in practical verifications. \<close>
-
-subsection*["law"::tc, main_author="Some(@{docitem ''lina''})"]
-\<open>\<^csp> Rules: Improved Proofs and New Results\<close>
-
-
-text\<open> The \<^csp> operators enjoy a number of algebraic properties: commutativity, 
-associativities, and idempotence in some cases. Moreover, there is a rich body of distribution
-laws between these operators. Our new version HOL-CSP 2 not only shortens and restructures the 
-proofs of @{cite "tej.ea:corrected:1997"}; the code reduces  
-to 8000 loc from 25000 loc. Some illustrative examples of new established rules are:
-
-  \<^item> \<open>\<box>x\<in>A\<union>B\<rightarrow>P(x) = (\<box>x\<in>A\<rightarrow>P x) \<box> (\<box>x\<in>B\<rightarrow>P x)\<close>
-  \<^item> \<open>A\<union>B\<subseteq>C \<Longrightarrow> (\<box>x\<in>A\<rightarrow>P x \<lbrakk>C\<rbrakk> \<box>x\<in>B\<rightarrow>Q x) = \<box>x\<in>A\<inter>B\<rightarrow>(P x \<lbrakk>C\<rbrakk> Q x)\<close>
-  \<^item> @{cartouche [display]\<open>A\<subseteq>C \<Longrightarrow> B\<inter>C={} \<Longrightarrow> 
-               (\<box>x\<in>A\<rightarrow>P x \<lbrakk>C\<rbrakk> \<box>x\<in>B\<rightarrow>Q x) = \<box>x\<in>B\<rightarrow>(\<box>x\<in>A\<rightarrow>P x \<lbrakk>C\<rbrakk> Q x)\<close>}
-  \<^item> \<open>finite A \<Longrightarrow> A\<inter>C = {} \<Longrightarrow> ((P \<lbrakk>C\<rbrakk> Q) \ A) = ((P \ A) \<lbrakk>C\<rbrakk> (Q \ A)) ...\<close>
-
- The continuity proof of the hiding operator is notorious. The proof is known
-to involve the classical König's lemma stating that every infinite tree with finite branching 
-has an infinite path. We adapt this lemma to our context as follows:
-
- @{cartouche [display, indent=5] 
- \<open>infinite tr \<Longrightarrow> \<forall>i. finite{t. \<exists>t'\<in>tr. t = take i t'} 
-             \<Longrightarrow> \<exists> f. strict_mono f \<and> range f \<subseteq> {t. \<exists>t'\<in>tr. t \<le> t'}\<close>}
-
-in order to come up with the continuity rule: \<open>finite S \<Longrightarrow> cont P \<Longrightarrow> cont(\<lambda>X. P X \ S)\<close>.
-The original proof had been drastically shortened by a factor 10 and important immediate steps
-generalized: monotonicity, for example, could be generalized to the infinite case. 
-
-As for new laws, consider the case of \<open>(P \ A) \ B = P \ (A \<union> B)\<close> which is 
-stated in @{cite "Roscoe:UCS:2010"} without proof. In the new version, we managed to establish 
-this law which still need 450 lines of complex Isar code. However, it turned out that the original
-claim is not fully true: it can only be established again by König's 
-lemma to build a divergent trace of  \<open>P \ (A \<union> B)\<close> which requires \<open>A\<close> to be finite 
-(\<open>B\<close> can be arbitrary) in order to use it from a divergent trace of  \<open>(P \ A) \ B\<close> 
-@{footnote \<open>In @{cite "Roscoe:UCS:2010"}, the authors point out that the laws involving the hiding 
-operator may fail when \<open>A\<close> is infinite; however, they fail to give the precise 
-conditions for this case.\<close>}. Again, we want to argue that the intricate number of
-cases to be considered as well as their complexity makes pen and paper proofs 
-practically infeasible.
-\<close>
-
-section*["newResults"::tc,main_author="Some(@{docitem ''safouan''}::author)",
-                                 main_author="Some(@{docitem ''lina''}::author)", level= "Some 3"]
-\<open>Theoretical Results on Refinement\<close>
-text\<open>\<close>
-subsection*["adm"::tc,main_author="Some(@{docitem ''safouan''}::author)", 
-                                  main_author="Some(@{docitem ''lina''}::author)"]
-\<open>Decomposition Rules\<close>
-text\<open>
-In our framework, we implemented the pcpo process refinement together with the five refinement 
-orderings introduced in @{technical "orderings"}. To enable fixed-point induction, we first have 
-the admissibility of the refinements.
-@{cartouche [display, indent=7] \<open>cont u \<Longrightarrow> mono v \<Longrightarrow> adm(\<lambda>x. u x \<sqsubseteq>\<^sub>\<FF> v x) where \<FF>\<in>{\<T>,\<F>,\<D>,\<T>\<D>,\<F>\<D>}\<close>}
-
-
-Next we analyzed the monotonicity of these refinement orderings, whose results are then used as 
-decomposition rules in our framework. 
-Some \<^csp> operators, such as multi-prefix and non-deterministic choice, are monotonic 
-under all refinement orderings, while others are not.    
-  
-\<^item> External choice is not monotonic only under \<open>\<sqsubseteq>\<^sub>\<F>\<close>, with the following monotonicities proved:
-  @{cartouche [display,indent=5]
-    \<open>P \<sqsubseteq>\<^sub>\<FF> P' \<Longrightarrow> Q \<sqsubseteq>\<^sub>\<FF> Q' \<Longrightarrow> (P \<box> Q) \<sqsubseteq>\<^sub>\<FF> (P' \<box> Q') where \<FF>\<in>{\<T>,\<D>,\<T>\<D>,\<F>\<D>}\<close>}
-\<^item> Sequence operator is not monotonic under \<open>\<sqsubseteq>\<^sub>\<F>\<close>, \<open>\<sqsubseteq>\<^sub>\<D>\<close> or \<open>\<sqsubseteq>\<^sub>\<T>\<close>:
-  @{cartouche [display,indent=5] 
-    \<open>P \<sqsubseteq>\<^sub>\<FF> P'\<Longrightarrow> Q \<sqsubseteq>\<^sub>\<FF> Q' \<Longrightarrow> (P ; Q) \<sqsubseteq>\<^sub>\<FF> (P' ; Q') where \<FF>\<in>{\<T>\<D>,\<F>\<D>}\<close>}
-%All refinements are right-side monotonic but \<open>\<sqsubseteq>\<^sub>\<F>\<close>, \<open>\<sqsubseteq>\<^sub>\<D>\<close> and \<open>\<sqsubseteq>\<^sub>\<T>\<close> are not left-side monotonic,
-%which can be explained by 
-%the interdependence relationship of failure and divergence projections for the first component. 
-%We thus proved:
-\<^item> Hiding operator is not monotonic under \<open>\<sqsubseteq>\<^sub>\<D>\<close>:
-  @{cartouche [display,indent=5] \<open>P \<sqsubseteq>\<^sub>\<FF> Q \<Longrightarrow> P \ A  \<sqsubseteq>\<^sub>\<FF> Q \ A where \<FF>\<in>{\<T>,\<F>,\<T>\<D>,\<F>\<D>}\<close>}
-%Intuitively, for the divergence refinement of the hiding operator, there may be
-%some trace \<open>s\<in>\<T> Q\<close> and \<open>s\<notin>\<T> P\<close> such that it becomes divergent in \<open>Q \ A\<close>  but 
-%not in \<open>P \ A\<close>.
-%when the condition in the corresponding projection laws is satisfied, which makes it is not monotonic.
-\<^item> Parallel composition is not monotonic under \<open>\<sqsubseteq>\<^sub>\<F>\<close>, \<open>\<sqsubseteq>\<^sub>\<D>\<close> or \<open>\<sqsubseteq>\<^sub>\<T>\<close>:
-  @{cartouche [display,indent=5] \<open>P \<sqsubseteq>\<^sub>\<FF> P' \<Longrightarrow> Q \<sqsubseteq>\<^sub>\<FF> Q' \<Longrightarrow> (P \<lbrakk>A\<rbrakk> Q) \<sqsubseteq>\<^sub>\<FF> (P' \<lbrakk>A\<rbrakk> Q') where \<FF>\<in>{\<T>\<D>,\<F>\<D>}\<close>}
-%The failure and divergence projections of this operator are also interdependent, similar to the 
-%sequence operator. 
-%Hence, this operator is not monotonic with \<open>\<sqsubseteq>\<^sub>\<F>\<close>, \<open>\<sqsubseteq>\<^sub>\<D>\<close> and \<open>\<sqsubseteq>\<^sub>\<T>\<close>, but monotonic when their 
-%combinations are considered. 
-
-\<close>
-
-(* Besides the monotonicity results on the above \<^csp> operators, 
-we have also proved that for other \<^csp> operators, such as multi-prefix and non-deterministic choice, 
-they are all monotonic with these five refinement orderings. Such theoretical results provide significant indicators 
-for semantics choices when considering specification decomposition. 
-We want to emphasize that this is the first work on such substantial 
-analysis in a formal way, as far as we know. 
-
-%In the literature, these processes are defined in a way that does not distinguish the special event \<open>tick\<close>. To be consistent with the idea that ticks should be distinguished on the semantic level, besides the above
-three processes,
-
-one can directly prove 3 since for both \<open>CHAOS\<close> and \<open>DF\<close>,
-the version with \<open>SKIP\<close> is constructed exactly in the same way from that without \<open>SKIP\<close>. 
-And 4 is obtained based on the projection laws of internal choice \<open>\<sqinter>\<close>.
-Finally, for 5, the difference between \<open>DF\<close> and \<open>RUN\<close> is that the former applies internal choice 
-while the latter with external choice. From the projection laws of both operators, 
-the failure set of \<open>RUN\<close> has more constraints, thus being a subset of that of \<open>DF\<close>, 
-when the divergence set is empty, which is true for both processes. 
-
-*)
-
-subsection*["processes"::tc,main_author="Some(@{docitem ''safouan''}::author)", 
-                            main_author="Some(@{docitem ''lina''}::author)"]
-\<open>Reference Processes and their Properties\<close>
-text\<open>
-We now present reference processes that exhibit basic behaviors, introduced in  
-fundamental \<^csp> works @{cite "Roscoe:UCS:2010"}. The process \<open>RUN A\<close> always 
-accepts events from \<open>A\<close> offered by the environment. The process \<open>CHAOS A\<close> can always choose to 
-accept or reject any event of \<open>A\<close>. The process \<open>DF A\<close> is the most non-deterministic deadlock-free 
-process on \<open>A\<close>, \<^ie>, it can never refuse all events of \<open>A\<close>. 
-To handle termination better, we added two new processes \<open>CHAOS\<^sub>S\<^sub>K\<^sub>I\<^sub>P\<close> and \<open>DF\<^sub>S\<^sub>K\<^sub>I\<^sub>P\<close>. 
-%Note that we do not redefine \<open>RUN\<close> with \<open>SKIP\<close> because this process is supposed to never terminate, 
-%thus must be without it. 
-\<close>
-
-(*<*) (* a test ...*)
-text*[X22 ::math_content   ]\<open>\<open>RUN A \<equiv> \<mu> X. \<box> x \<in> A \<rightarrow> X\<close>                           \<close>
-text*[X32::"definition", mcc=defn]\<open>\<open>CHAOS A \<equiv> \<mu> X. (STOP \<sqinter> (\<box> x \<in> A \<rightarrow> X))\<close>        \<close>
-Definition*[X42]\<open>\<open>CHAOS\<^sub>S\<^sub>K\<^sub>I\<^sub>P A \<equiv> \<mu> X. (SKIP \<sqinter> STOP \<sqinter> (\<box> x \<in> A \<rightarrow> X))\<close>  \<close>
-Definition*[X52::"definition"]\<open>\<open>CHAOS\<^sub>S\<^sub>K\<^sub>I\<^sub>P A \<equiv> \<mu> X. (SKIP \<sqinter> STOP \<sqinter> (\<box> x \<in> A \<rightarrow> X))\<close> \<close>
-
-text\<open> The \<open>RUN\<close>-process defined @{math_content X22} represents the process that accepts all 
-events, but never stops nor deadlocks. The \<open>CHAOS\<close>-process comes in two variants shown in 
-@{definition X32} and @{definition X42} @{definition X52}: the process that non-deterministically 
-stops or accepts any offered event, whereas \<open>CHAOS\<^sub>S\<^sub>K\<^sub>I\<^sub>P\<close> can additionally terminate.\<close>
-(*>*)
-
-Definition*[X2]\<open>\<open>RUN A \<equiv> \<mu> X. \<box> x \<in> A \<rightarrow> X\<close>                    \<close>
-Definition*[X3]\<open>\<open>CHAOS A \<equiv> \<mu> X. (STOP \<sqinter> (\<box> x \<in> A \<rightarrow> X))\<close>         \<close>
-Definition*[X4]\<open>\<open>CHAOS\<^sub>S\<^sub>K\<^sub>I\<^sub>P A \<equiv> \<mu> X. (SKIP \<sqinter> STOP \<sqinter> (\<box> x \<in> A \<rightarrow> X))\<close>\<close>
-Definition*[X5]\<open>\<open>DF A \<equiv> \<mu> X. (\<sqinter> x \<in> A \<rightarrow> X)\<close>                       \<close>
-Definition*[X6]\<open>\<open>DF\<^sub>S\<^sub>K\<^sub>I\<^sub>P A \<equiv> \<mu> X. ((\<sqinter> x \<in> A \<rightarrow> X) \<sqinter> SKIP)\<close>          \<close> 
-
-text\<open>In the following, we denote \<open> \<R>\<P> = {DF\<^sub>S\<^sub>K\<^sub>I\<^sub>P, DF, RUN, CHAOS, CHAOS\<^sub>S\<^sub>K\<^sub>I\<^sub>P}\<close>. 
-All five  reference processes are divergence-free.
-%which was done by using a particular lemma \<open>\<D> (\<mu> x. f x) = \<Inter>\<^sub>i\<^sub>\<in>\<^sub>\<nat> \<D> (f\<^sup>i \<bottom>)\<close>.  
-@{cartouche 
-  [display,indent=8] \<open> D (\<PP> UNIV) = {} where \<PP> \<in> \<R>\<P> and UNIV is the set of all events\<close>
-}
-Regarding the failure refinement ordering, the set of failures \<open>\<F> P\<close> for any process \<open>P\<close> is
-a subset of  \<open>\<F> (CHAOS\<^sub>S\<^sub>K\<^sub>I\<^sub>P UNIV)\<close>.% and the following lemma was proved: 
-% This proof is performed by induction, based on the failure projection of \<open>STOP\<close> and that of 
-% internal choice.
-
-
-   @{cartouche [display, indent=25] \<open>CHAOS\<^sub>S\<^sub>K\<^sub>I\<^sub>P UNIV \<sqsubseteq>\<^sub>\<F> P\<close>}
-
-
-\<^noindent> Furthermore, the following 5 relationships were demonstrated from monotonicity results and 
-a denotational proof.  
-%among which 1 and 2 are immediate corollaries, 
-%4 and 5 are directly obtained from our monotonicity results while 3 requires a denotational proof.
-and thanks to transitivity, we can derive other relationships.
-
-
-  \<^enum> \<open>CHAOS\<^sub>S\<^sub>K\<^sub>I\<^sub>P A \<sqsubseteq>\<^sub>\<F> CHAOS A\<close>
-  \<^enum> \<open>CHAOS\<^sub>S\<^sub>K\<^sub>I\<^sub>P A \<sqsubseteq>\<^sub>\<F> DF\<^sub>S\<^sub>K\<^sub>I\<^sub>P A\<close>  
-  \<^enum> \<open>CHAOS A \<sqsubseteq>\<^sub>\<F> DF A\<close>
-  \<^enum> \<open>DF\<^sub>S\<^sub>K\<^sub>I\<^sub>P A \<sqsubseteq>\<^sub>\<F> DF A\<close>  
-  \<^enum> \<open>DF A \<sqsubseteq>\<^sub>\<F> RUN A\<close>  
-
-
-Last, regarding trace refinement, for any process P, 
-its set of traces \<open>\<T> P\<close> is a subset of  \<open>\<T> (CHAOS\<^sub>S\<^sub>K\<^sub>I\<^sub>P UNIV)\<close> and of  \<open>\<T> (DF\<^sub>S\<^sub>K\<^sub>I\<^sub>P UNIV)\<close> as well.
-%As we already proved that \<open>CHAOS\<^sub>S\<^sub>K\<^sub>I\<^sub>P\<close> covers all failures, 
-%we can immediately infer that it also covers all traces. 
-%The \<open>DF\<^sub>S\<^sub>K\<^sub>I\<^sub>P\<close> case requires a longer denotational proof.
-
-
-  \<^enum> \<open>CHAOS\<^sub>S\<^sub>K\<^sub>I\<^sub>P UNIV \<sqsubseteq>\<^sub>\<T> P\<close>
-  \<^enum> \<open>DF\<^sub>S\<^sub>K\<^sub>I\<^sub>P UNIV \<sqsubseteq>\<^sub>\<T> P\<close>
-
-\<close>
-
-text\<open> 
-Recall that a concurrent system is considered as being deadlocked if no component can make any 
-progress,  caused for example by the competition for resources. In opposition to deadlock, 
-processes can enter infinite loops inside a sub-component without never ever interact with their 
-environment again  ("infinite internal chatter"); this situation called  divergence or livelock. 
-Both properties are not just a sanity condition; in \<^csp>, they play a central role for 
-verification. For example, if one wants to establish that a protocol implementation \<open>IMPL\<close> satisfies 
-a non-deterministic specification \<open>SPEC\<close> it suffices to ask if \<open>IMPL || SPEC\<close> is deadlock-free.
-In this setting, \<open>SPEC\<close> becomes a kind of observer that signals non-conformance of \<open>IMPL\<close> by 
-deadlock.
-% A livelocked system looks similar to a deadlocked one from an external point of view. 
-% However, livelock is sometimes considered as worse since the user may be able to observe the internal 
-% activities and so hope that some output will happen eventually. 
-
-In the literature, deadlock and lifelock are phenomena that are often 
-handled separately. One contribution of our work is establish their precise relationship inside
-the Failure/Divergence Semantics of \<^csp>.\<close>
-
-(* bizarre: Definition* does not work for this single case *)
-text*[X10::"definition"]\<open> \<open>deadlock\<^sub>-free P \<equiv>  DF\<^sub>S\<^sub>K\<^sub>I\<^sub>P UNIV \<sqsubseteq>\<^sub>\<F> P\<close>  \<close>
-
-text\<open>\<^noindent> A process \<open>P\<close> is deadlock-free if and only if after any trace \<open>s\<close> without \<open>\<surd>\<close>, the union of \<open>\<surd>\<close> 
-and all events of \<open>P\<close> can never be a refusal set associated to \<open>s\<close>, which means that \<open>P\<close> cannot 
-be deadlocked after any non-terminating trace.   
-\<close>
-
-Theorem*[T1, short_name="\<open>DF definition captures deadlock-freeness\<close>"]
-\<open> \hfill \break \<open>deadlock_free P \<longleftrightarrow> (\<forall>s\<in>\<T> P. tickFree s \<longrightarrow> (s, {\<surd>}\<union>events_of P) \<notin> \<F> P)\<close> \<close>   
-Definition*[X11]\<open>  \<open>livelock\<^sub>-free P \<equiv> \<D> P = {} \<close>   \<close>
-
-text\<open> Recall that all five reference processes are livelock-free. 
-We also have the following lemmas about the 
-livelock-freeness of processes: 
-  \<^enum> \<open>livelock\<^sub>-free P \<longleftrightarrow> \<PP> UNIV \<sqsubseteq>\<^sub>\<D> P where \<PP> \<in> \<R>\<P>\<close> 
-  \<^enum> @{cartouche [display]\<open>livelock\<^sub>-free P \<longleftrightarrow> DF\<^sub>S\<^sub>K\<^sub>I\<^sub>P UNIV \<sqsubseteq>\<^sub>\<T>\<^sub>\<D> P 
-                    \<longleftrightarrow> CHAOS\<^sub>S\<^sub>K\<^sub>I\<^sub>P UNIV \<sqsubseteq>\<^sub>\<T>\<^sub>\<D> P\<close>}
-  \<^enum> \<open>livelock\<^sub>-free P \<longleftrightarrow> CHAOS\<^sub>S\<^sub>K\<^sub>I\<^sub>P UNIV \<sqsubseteq>\<^sub>\<F>\<^sub>\<D> P\<close> 
-\<close>
-text\<open>
-Finally, we proved the following theorem that confirms the relationship between the two vital
-properties:
-\<close>
-Theorem*[T2, short_name="''DF implies LF''"]
-  \<open>  \<open>deadlock_free P \<longrightarrow> livelock_free P\<close>   \<close>
-
-text\<open>
-This is totally natural, at a first glance, but surprising as the proof of deadlock-freeness only 
-requires failure refinement \<open>\<sqsubseteq>\<^sub>\<F>\<close> (see @{definition \<open>X10\<close>}) where divergence traces are mixed within 
-the failures set. Note that the existing tools in the literature normally detect these two phenomena  
-separately, such as FDR for which checking livelock-freeness is very costly. 
-In our framework, deadlock-freeness of a given system 
-implies its livelock-freeness. However, if a system is not deadlock-free, 
-then it may still be livelock-free. % This makes sense since livelocks are worse than deadlocks.   
-
-\<close>
-
-section*["advanced"::tc,main_author="Some(@{docitem ''safouan''}::author)",level="Some 3"]
-\<open>Advanced Verification Techniques\<close>
-
-text\<open>
- Based on the refinement framework discussed in @{docitem "newResults"}, we will now
-turn to some more advanced proof principles, tactics and verification techniques. 
-We will demonstrate them on two paradigmatic examples well-known in the \<^csp> literature: 
-The CopyBuffer and Dijkstra's Dining Philosophers. In both cases, we will exploit 
-the fact that HOL-CSP 2 allows for reasoning over infinite \<^csp>; in the first case,
-we reason over infinite alphabets approaching an old research objective:
-exploiting data-independence @{cite "Lazic1998ASS" and "AnZhangYou14"} in process
-verification. In the latter case, we present an approach to a verification of a parameterized 
-architecture, in this case a ring-structure of arbitrary size.
-\<close>
-
-subsection*["illustration"::tc,main_author="Some(@{docitem ''safouan''}::author)", level="Some 3"]
-\<open>The General CopyBuffer Example\<close>
-text\<open>
-We consider the paradigmatic copy buffer example @{cite "Hoare:1985:CSP:3921" and "Roscoe:UCS:2010"} 
-that is characteristic for a specification of a  prototypical process and its
- implementation. It is used extensively in the \<^csp> literature to illustrate the interplay 
-of communication, component concealment and fixed-point operators.
-The process \<open>COPY\<close> is a specification of a one size buffer, that receives elements from the channel 
-\<open>left\<close> of arbitrary type \<open>\<alpha>\<close> and outputs them on the channel \<open>right\<close>: 
-
-@{theory_text [display,indent=5] \<open>
-datatype  \<alpha> events = left \<alpha> | right \<alpha> | mid \<alpha> | ack
-definition COPY \<equiv> (\<mu> X. left?x \<rightarrow> (right!x \<rightarrow> X))\<close>}
-
- \<^noindent> From our HOL-CSP 2 theory that establishes the continuity of all \<^csp> operators, we deduce that 
-such a fixed-point process \<open>COPY\<close> exists and follows the unrolling rule below: 
-
-@{theory_text [display,indent=5] \<open>lemma COPY = (left?x \<rightarrow> (right!x \<rightarrow> COPY))\<close>}
-
- \<^noindent> We set \<open>SEND\<close> and \<open>REC\<close> in parallel but in a row sharing a middle channel 
-\<open>mid\<close> and synchronizing with an \<open>ack\<close> event. Then, we hide all exchanged events between these two 
-processes and we call the resulting process \<open>SYSTEM\<close>: 
-
-@{theory_text [display,indent=5] \<open>
-definition SEND \<equiv> (\<mu> X. left?x \<rightarrow> (mid!x \<rightarrow> (ack \<rightarrow> X)))
-definition REC  \<equiv> (\<mu> X. mid?x \<rightarrow> (right!x \<rightarrow> (ack \<rightarrow> X)))
-definition SYN  \<equiv> (range mid) \<union> {ack}
-definition "SYSTEM \<equiv> (SEND \<lbrakk>SYN\<rbrakk> REC) \\ SYN"\<close>}
-
- \<^noindent> We want to verify that \<open>SYSTEM\<close> implements \<open>COPY\<close>. As shown below, we apply fixed-point induction 
-to prove that \<open>SYSTEM\<close> refines \<open>COPY\<close> using the \<open>pcpo\<close> process ordering \<open>\<sqsubseteq>\<close> that implies all other 
-refinement orderings. We state: 
-
-@{theory_text [display,indent=5] \<open>lemma: COPY \<sqsubseteq> SYSTEM\<close>} 
-
-and apply fixed-point induction over \<open>COPY\<close>; this leaves us to the three subgoals: 
-  \<^enum> \<open>adm (\<lambda>a. a \<sqsubseteq> (SEND \<lbrakk>SYN\<rbrakk> REC) \ SYN)\<close>
-  \<^enum> \<open>\<bottom> \<sqsubseteq> (SEND \<lbrakk>SYN\<rbrakk> REC) \ SYN\<close>
-  \<^enum> @{cartouche [display]\<open>P \<sqsubseteq> (SEND \<lbrakk>SYN\<rbrakk> REC) \ SYN \<Longrightarrow> 
-                              left?x \<rightarrow> right!x \<rightarrow> P \<sqsubseteq> (SEND \<lbrakk>SYN\<rbrakk> REC) \ SYN\<close>} 
-
-The first two sub-proofs are automatic simplification proofs; the third requires unfolding
-\<open>SEND\<close> and \<open>REC\<close> one step and applying the algebraic laws. No denotational
-semantics reasoning is necessary here; it is just an induct-simplify proof consisting
-of 2 lines proof-script involving the derived algebraic laws of \<^csp>.
-
-After proving that \<open>SYSTEM\<close> implements \<open>COPY\<close> for arbitrary alphabets, we aim to profit from this 
-first established result to check which relations \<open>SYSTEM\<close> has wrt. to the reference processes of 
-@{docitem "processes"}. Thus, we prove that \<open>COPY\<close> is deadlock-free which implies livelock-free, 
-(proof by fixed-induction  similar to \<open>lemma: COPY \<sqsubseteq> SYSTEM\<close>), from which we can immediately infer 
-from transitivity that \<open>SYSTEM\<close> is. Using refinement relations, we killed four birds with one stone 
-as we proved the deadlock-freeness and  the livelock-freeness for both \<open>COPY\<close> and \<open>SYSTEM\<close> processes. 
-These properties hold for arbitrary alphabets and for infinite ones in particular.
- 
-@{theory_text [display, indent=5] \<open>
-lemma DF UNIV \<sqsubseteq> COPY
-
-corollary deadlock_free COPY
-      and livelock_free COPY
-      and deadlock_free SYSTEM
-      and livelock_free SYSTEM\<close>}
-
-\<close>
-
-
-subsection*["inductions"::tc,main_author="Some(@{docitem ''safouan''}::author)"]
-\<open>New Fixed-Point Inductions\<close>
-
-text\<open>
- The copy buffer refinement proof \<open>DF UNIV \<sqsubseteq> COPY\<close> is a typical one step induction proof 
-with two goals:
-\<open>base: \<bottom> \<sqsubseteq> Q\<close> and \<open>1-ind: X \<sqsubseteq> Q \<Longrightarrow> (_ \<rightarrow> X) \<sqsubseteq> Q\<close>. Now, if unfolding the fixed-point process \<open>Q\<close> 
-reveals two steps, the second goal becomes 
-\<open>X \<sqsubseteq> Q \<Longrightarrow> _ \<rightarrow> X \<sqsubseteq> _ \<rightarrow> _ \<rightarrow> Q\<close>. Unfortunately, this way, it becomes improvable 
-using monotonicities rules. 
-We need here a two-step induction of the form \<open>base0: \<bottom> \<sqsubseteq> Q\<close>, \<open>base1: _ \<rightarrow> \<bottom> \<sqsubseteq> Q\<close> and 
-\<open>2-ind: X \<sqsubseteq> Q \<Longrightarrow> _ \<rightarrow>  _ \<rightarrow> X \<sqsubseteq> _ \<rightarrow> _ \<rightarrow> Q\<close> to have a sufficiently powerful induction scheme.
-
-For this reason, we derived a number of alternative induction schemes (which are not available
-in the HOLCF library), which are also relevant for our final Dining Philophers example.
-These are essentially adaptions of k-induction schemes applied to domain-theoretic
-setting (so: requiring \<open>f\<close> continuous and \<open>P\<close> admissible; these preconditions are
-skipped here): 
-  \<^item> @{cartouche [display]\<open>... \<Longrightarrow> \<forall>i<k. P (f\<^sup>i \<bottom>) \<Longrightarrow> (\<forall>X. (\<forall>i<k. P (f\<^sup>i X)) \<longrightarrow> P (f\<^sup>k X)) 
-      \<Longrightarrow> P (\<mu>X. f X)\<close>}
-  \<^item> \<open>... \<Longrightarrow> \<forall>i<k. P (f\<^sup>i \<bottom>) \<Longrightarrow> (\<forall>X. P X \<longrightarrow> P (f\<^sup>k X)) \<Longrightarrow> P (\<mu>X. f X)\<close>
-
-
-\<^noindent> In the latter variant, the induction hypothesis is weakened to skip \<open>k\<close> steps. When possible,
-it reduces the goal size.
-
-Another problem occasionally occurring in refinement proofs happens when the right side term 
-involves more than one  fixed-point  process (\<^eg> \<open>P \<lbrakk>{A}\<rbrakk> Q \<sqsubseteq> S\<close>). In this situation,
-we need parallel fixed-point inductions. The HOLCF library offers only a basic one:
-  \<^item> @{cartouche [display]\<open>... \<Longrightarrow> P \<bottom> \<bottom> \<Longrightarrow> (\<forall>X Y. P X Y \<Longrightarrow> P (f X) (g Y)) 
-        \<Longrightarrow> P (\<mu>X. f X) (\<mu>X. g X)\<close>}
-
-
-\<^noindent> This form does not help in cases like in \<open>P \<lbrakk>\<emptyset>\<rbrakk> Q \<sqsubseteq> S\<close> with the interleaving operator on the 
-right-hand side. The simplifying law is:
-@{cartouche [display, indent=3]\<open>
-(\<box>x\<in>A\<rightarrow>P x \<lbrakk>\<emptyset>\<rbrakk> \<box>x\<in>B\<rightarrow>Q x) =   (\<box>x\<in>A \<rightarrow> (            P x \<lbrakk>\<emptyset>\<rbrakk> \<box>x\<in>B \<rightarrow> Q x) 
-                                         \<box> (\<box>x\<in>B \<rightarrow> (\<box>x\<in>A \<rightarrow> P x \<lbrakk>\<emptyset>\<rbrakk>          Q x))\<close>}
-Here, \<open>(f X \<lbrakk>\<emptyset>\<rbrakk> g Y)\<close> does not reduce to the \<open>(X \<lbrakk>\<emptyset>\<rbrakk> Y)\<close> term but to two terms \<open>(f X \<lbrakk>\<emptyset>\<rbrakk> Y)\<close> and 
-\<open>(X \<lbrakk>\<emptyset>\<rbrakk> g Y)\<close>.
-To handle these cases, we developed an advanced parallel induction scheme and we proved its 
-correctness:
-  \<^item> @{cartouche [display] \<open>... \<Longrightarrow> (\<forall>Y. P \<bottom> Y) \<Longrightarrow> (\<forall>X. P X \<bottom>)
-     \<Longrightarrow> \<forall>X Y. (P X Y \<and> P (f X) Y \<and> P X (g Y)) \<longrightarrow> P (f X) (g Y) 
-      \<Longrightarrow> P (\<mu>X. f X) (\<mu>X. g X)\<close>}
-
-
-\<^noindent> which allows for a "independent unroling" of the fixed-points in these proofs.
-The astute reader may notice here that if the induction step is weakened (having more hypothesises), 
-the base steps require enforcement.  
-\<close>
-
-subsection*["norm"::tc,main_author="Some(@{docitem ''safouan''}::author)"]
-\<open>Normalization\<close>
-text\<open>
- Our framework can reason not only over infinite alphabets, but also over processes parameterized
-over states with an arbitrarily rich structure. This  paves the way for the following technique, 
-that trades potentially complex process structure against equivalent simple processes with 
-potentially rich state.
-
-Roughly similar to labelled transition systems, we provide for deterministic \<^csp> processes a normal 
-form that is based on an explicit state. The general schema of normalized processes is defined as 
-follows:
-
-@{cartouche [display,indent=20] \<open>P\<^sub>n\<^sub>o\<^sub>r\<^sub>m\<lbrakk>\<tau>\<^sub>,\<upsilon>\<rbrakk> \<equiv> \<mu> X. (\<lambda>\<sigma>. \<box>e\<in>(\<tau> \<sigma>) \<rightarrow> X(\<upsilon> \<sigma> e))\<close>}
- where \<open>\<tau>\<close> is a transition function which returns the set of events that can be triggered from 
-the current  state \<open>\<sigma>\<close> given as parameter.
-The update function \<open>\<upsilon>\<close> takes two parameters \<open>\<sigma>\<close> and an event \<open>e\<close> and returns the new state.
-This normal form is closed under deterministic and  communication operators. 
-
-The advantage of this format is that we can mimick the well-known product automata construction
-for an arbitrary number of synchronized processes under normal form.
-We only show the case of the synchronous product of two processes: \<close>
-text*[T3::"theorem", short_name="\<open>Product Construction\<close>"]\<open>
-Parallel composition translates to normal form:
-@{cartouche [display,indent=5]\<open>(P\<^sub>n\<^sub>o\<^sub>r\<^sub>m\<lbrakk>\<tau>\<^sub>1,\<upsilon>\<^sub>1\<rbrakk> \<sigma>\<^sub>1) || (P\<^sub>n\<^sub>o\<^sub>r\<^sub>m\<lbrakk>\<tau>\<^sub>2,\<upsilon>\<^sub>2\<rbrakk> \<sigma>\<^sub>2) = 
-    P\<^sub>n\<^sub>o\<^sub>r\<^sub>m\<lbrakk>\<lambda>(\<sigma>\<^sub>1,\<sigma>\<^sub>2). \<tau>\<^sub>1 \<sigma>\<^sub>1 \<inter> \<tau>\<^sub>2 \<sigma>\<^sub>2 , \<lambda>(\<sigma>\<^sub>1,\<sigma>\<^sub>2).\<lambda>e.(\<upsilon>\<^sub>1 \<sigma>\<^sub>1 e, \<upsilon>\<^sub>2 \<sigma>\<^sub>2 e)\<rbrakk> (\<sigma>\<^sub>1,\<sigma>\<^sub>2)\<close>}
-\<close>
-
-text\<open> The generalization of this rule for a list of \<open>(\<tau>,\<upsilon>)\<close>-pairs is straight-forward, 
-albeit the formal  proof is not. The application of the generalized  form is a corner-stone of the 
-proof of the general dining philosophers problem illustrated in the subsequent section.
-
-Another advantage of normalized processes is the possibility to argue over the reachability of 
-states via the closure \<open>\<RR>\<close>, which is defined inductively over: 
-
-  \<^item> \<open>\<sigma> \<in> \<RR> \<tau> \<upsilon> \<sigma>\<close>
-  \<^item> \<open>\<sigma> \<in> \<RR> \<tau> \<upsilon> \<sigma>\<^sub>0 \<Longrightarrow> e \<in> \<tau> \<sigma> \<Longrightarrow> \<upsilon> \<sigma> e \<in> \<RR> \<tau> \<upsilon> \<sigma>\<^sub>0\<close>
-
-
-Thus, normalization leads to a new characterization of deadlock-freeness inspired 
-from automata theory. We formally proved the following theorem:\<close>
-
-text*[T4::"theorem", short_name="\<open>DF vs. Reacheability\<close>"]
-\<open> If each reachable state \<open>s \<in> (\<RR> \<tau> \<upsilon>)\<close> has outgoing transitions,
-the \<^csp> process is deadlock-free: 
-@{cartouche [display,indent=10] \<open>\<forall>\<sigma> \<in> (\<RR> \<tau> \<upsilon> \<sigma>\<^sub>0). \<tau> \<sigma> \<noteq> {} \<Longrightarrow> deadlock_free (P\<^sub>n\<^sub>o\<^sub>r\<^sub>m\<lbrakk>\<tau>,\<upsilon>\<rbrakk> \<sigma>\<^sub>0)\<close>}
-\<close>
-
-text\<open>  This theorem allows for establishing properties such as deadlock-freeness by 
-completely abstracting from \<^csp> theory; these are arguments that only involve inductive reasoning 
-over the transition function. 
-
-Summing up, our method consists of four stages:
-\<^enum>  we construct normalized versions of component processes and prove them
-  equivalent to their counterparts,
-\<^enum> we state an invariant over the states/variables,
-\<^enum> we prove by induction over \<open>\<RR>\<close> that it holds on all reachable states, and finally
-\<^enum> we prove that this invariant guarantees the existence of outgoing transitions.
-
-\<close>
-
-subsection*["dining_philosophers"::tc,main_author="Some(@{docitem ''safouan''}::author)",level="Some 3"]
-\<open>Generalized Dining Philosophers\<close>
-
-text\<open>  The dining philosophers problem is another paradigmatic example in the \<^csp> literature
-often used to illustrate synchronization problems between an arbitrary number of concurrent systems. 
-It is an example for a process scheme for which general properties are desirable in order
-to inherit them for specific instances.
-The general dining philosopher problem for an arbitrary \<open>N\<close> is presented in HOL-CSP 2 as follows
-%@{footnote \<open>The dining philosopher problem is also distributed with FDR4, where \<open>N = 6\<close>.\<close>}:
-
-@{theory_text [display,indent=5] 
-\<open>datatype dining_event  = picks (phil::nat) (fork::nat) 
-                             | putsdown (phil::nat) (fork::nat)
-                             | eat (phil::nat)
-definition LPHIL0  \<equiv> (\<mu> X. (picks 0 (N-1) \<rightarrow> (picks 0 0 \<rightarrow> eat 0 \<rightarrow>
-                                   (putsdown 0 0 \<rightarrow> (putsdown 0 (N-1) \<rightarrow> X)))))
-definition RPHIL i \<equiv> (\<mu> X. (picks i i \<rightarrow> (picks i (i-1) \<rightarrow> eat i \<rightarrow>
-                                   (putsdown i (i-1) \<rightarrow> (putsdown i i \<rightarrow> X)))))
-definition FORK i  \<equiv> (\<mu> X.   (picks i i \<rightarrow> (putsdown i i \<rightarrow> X)) 
-                                   \<box>(picks (i+1)%N i \<rightarrow>(putsdown (i+1)%N i \<rightarrow> X)))
-definition "PHILs   \<equiv> LPHIL0 ||| (|||\<^sub>i\<^sub>\<in>\<^sub>1\<^sub>.\<^sub>.\<^sub>N RPHIL i)" 
-definition "FORKs   \<equiv> |||\<^sub>i\<^sub>\<in>\<^sub>0\<^sub>.\<^sub>.\<^sub>N FORK i"
-definition DINING  \<equiv> FORKs \<lbrakk>picks, putsdown\<rbrakk> PHILs\<close>}
-
-% this should be theory_text, but is rejected for lexical reasons
-Note that both philosophers and forks are pairwise independent 
-but both synchronize on \<open>picks\<close> and \<open>putsdown\<close> events. The philosopher of index 0 is left-handed 
-whereas the other \<open>N-1\<close> philosophers are right-handed. We want to prove that any configuration 
-is deadlock-free for an arbitrary number N.
-
-First, we put the fork process under normal form. It has three states:
-(1) on the table, (2) picked by the right philosopher or (3) picked by the left one:
-
-@{theory_text [display,indent=5]
-\<open>definition trans\<^sub>f i \<sigma> \<equiv> if       \<sigma> = 0   then {picks i i, picks (i+1)%N i}
-                             else if \<sigma> = 1   then {putsdown i i} 
-                             else if \<sigma> = 2   then {putsdown (i+1)%N i}
-                             else                     {}
-definition upd\<^sub>f i \<sigma> e \<equiv> if       e = (picks i i)           then 1 
-                              else if e = (picks (i+1)%N) i then 2 
-                              else                                        0
-definition FORK\<^sub>n\<^sub>o\<^sub>r\<^sub>m i \<equiv> P\<^sub>n\<^sub>o\<^sub>r\<^sub>m\<lbrakk>trans\<^sub>f i, upd\<^sub>f i\<rbrakk> \<close>}
-
-To validate our choice for the states, transition function \<open>trans\<^sub>f\<close> and update function \<open>upd\<^sub>f\<close>,
-we prove that they are equivalent to the original process components: \<open>FORK\<^sub>n\<^sub>o\<^sub>r\<^sub>m i = FORK i\<close>. 
-The anti-symmetry of refinement breaks this down to the two refinement proofs \<open>FORK\<^sub>n\<^sub>o\<^sub>r\<^sub>m i \<sqsubseteq> FORK i\<close> 
-and \<open>FORK i \<sqsubseteq> FORK\<^sub>n\<^sub>o\<^sub>r\<^sub>m i\<close>, which are similar to the CopyBuffer example shown in 
-@{technical "illustration"}. Note, again, that this fairly automatic induct-simplify-proof just 
-involves reasoning on the derived algebraic rules, not any reasoning on the level of the 
-denotational semantics. 
-
-%Second we prove that the normal form process is equivalent to the original fork process 
-%by proving refinements in both directions. We note here that the first refinement \<open>FORK\<^sub>n\<^sub>o\<^sub>r\<^sub>m i \<sqsubseteq> FORK i\<close> 
-%requires a two steps induction as unfolding the original fixed-point process brings two steps 
-%\<open>FORK i = picks \<rightarrow> putsdown \<rightarrow> FORK i\<close>. After that we apply the same method 
-%to get the philosopher process under a normal form.
-
-Thanks to @{theorem \<open>T3\<close>}, we obtain normalized processes 
-for \<open>FORKs\<close>, \<open>PHILs\<close> and \<open>DINING\<close>:
-@{theory_text [display,indent=5] 
-\<open>definition "trans\<^sub>F \<equiv> \<lambda>fs. (\<Inter>\<^sub>i\<^sub><\<^sub>N. trans\<^sub>f i (fs!i))"
-definition upd\<^sub>F   \<equiv> \<lambda>fs e. let i=(fork e) in fs[i:=(upd\<^sub>f i (fs!i) e)]
-
-lemma FORKs = P\<^sub>n\<^sub>o\<^sub>r\<^sub>m\<lbrakk>trans\<^sub>F, upd\<^sub>F\<rbrakk> ...
-lemma PHILS = P\<^sub>n\<^sub>o\<^sub>r\<^sub>m\<lbrakk>trans\<^sub>P, upd\<^sub>P\<rbrakk> ...
-
-definition trans\<^sub>D \<equiv> \<lambda>(ps,fs). (trans\<^sub>P ps) \<inter> (trans\<^sub>F fs)
-definition upd\<^sub>D   \<equiv> \<lambda>(ps,fs) e. (upd\<^sub>P ps e, upd\<^sub>F fs e)
-
-lemma DINING = P\<^sub>n\<^sub>o\<^sub>r\<^sub>m\<lbrakk>trans\<^sub>D, upd\<^sub>D\<rbrakk> \<close>}
-The variable \<open>ps\<close> stands for the list of philosophers states and \<open>fs\<close> 
-for the list of forks states, both are of size \<open>N\<close>. The pair \<open>(ps, fs)\<close> 
-encodes the whole dining table state over which we need to define an invariant to ensure 
-that no blocking state is reachable and thus the dining philosophers problem is deadlock-free.
-As explained before, the proof is based on abstract reasoning over relations 
-independent from the \<^csp> context.
-
-The last steps towards our goal are the following definitions and lemmas:
-
-@{theory_text [display,indent=5]
-\<open>definition INV\<^sub>D\<^sub>I\<^sub>N\<^sub>I\<^sub>N\<^sub>G ps fs \<equiv> (\<forall>i. ((fs!i=1) \<leftrightarrow> ps!i \<noteq> 0) \<and> ... )
-lemma (ps,fs) \<in> \<RR> trans\<^sub>D upd\<^sub>D  \<Longrightarrow> INV\<^sub>D\<^sub>I\<^sub>N\<^sub>I\<^sub>N\<^sub>G ps fs ...
-lemma INV\<^sub>D\<^sub>I\<^sub>N\<^sub>I\<^sub>N\<^sub>G ps fs \<Longrightarrow> trans\<^sub>D (ps, fs) \<noteq> {} ...
-
-corollary deadlock_free DINING \<close>} 
-
-To sum up, we proved once and for all that the dining philosophers problem is deadlock free 
-for an arbitrary number \<open>N \<ge> 2\<close>. Common model-checkers like PAT and FDR fail to answer 
-for a dozen of philosophers (on a usual machine) due to the exponential combinatorial explosion.
-Furthermore, our proof is fairly stable against modifications like adding non synchronized events like
-thinking or sitting down in contrast to model-checking techniques. \<close>
-
-section*["relatedwork"::tc,main_author="Some(@{docitem ''lina''}::author)",level="Some 3"]
-\<open>Related work\<close>
-
-text\<open>
-The theory of \<^csp> has attracted a lot of interest from the eighties on, and is still
-a fairly active research area, both
-as a theoretical device as well as a modelling language to analyze complex concurrent systems. 
-It is therefore not surprising that attempts to its formalisation had been undertaken early
-with the advent of interactive theorem proving systems supporting higher-order logic 
- @{cite "Camilleri91" and "tej.ea:corrected:1997" and "10.1007/978-3-642-16690-7_9" 
-   and "10.1007/978-3-642-27705-4_20"  and "DBLP:conf/concur/IsobeR06" }, where
- especially the latter allows for some automated support for refinement proofs 
-based on induction. However, HOL-CSP2 is based on a failure/divergence model, while 
-@{cite "DBLP:conf/concur/IsobeR06"} is  based on stable failures, which can infer 
-deadlock-freeness only under the assumption that no lifelock occurred; In our view, 
-this is a too strong assumption for both the theory as well as the tool.
-
-In the 90ies, research focused on automated verification tools for \<^csp>, most notably on
-FDR~@{cite "fdr4"}. It relies on an operational \<^csp> semantics, allowing for a conversion of processes 
-into labelled transition systems, where the states are normalized by the "laws" derived from the 
-denotational semantics.
-For finite event sets, refinement proofs can be reduced to graph inclusion problems. With 
-efficient compression techniques, such as bisimulation, elimination and factorization by 
-semantic equivalence @{cite "Roscoe95"}, FDR was used to analyze some industrial applications. 
-However, such a model checker can not handle infinite cases and do not scale to large systems. 
-%%Another similar model checking tool @{cite "SunLDP09"} implemented some more optimization techniques, 
-%%such as partial order reduction, symmetric reduction, and parallel model checking, but is also 
-%%restricted to the finite case. 
-
-The fundamental limits of  automated decision procedures for data and processes has been known
-very early on: Undecidability of parameterized model checking was proven by reduction to 
-non-halting of Turing machines @{cite "Suzuki88"}. However, some forms of 
-well-structured transitions systems, could be demonstrated to be decidable 
-@{cite "FinkelS01" and "BloemJKKRVW16"}.
-HOL-CSP2 is a fully abstract model for the failure/divergence model; as a HOL theory, it is therefore
-a "relative complete proof theory" both for infinite data as well as number of components.
-(see @{cite "andrews2002introduction"} for relative completeness).
-
-
-Encouraged by the progress of SMT solvers which support some infinite types, 
-notably (fixed arrays of) integers or reals, and limited forms of formulas over these types,
-SMT-based model-checkers represent the current main-stream to parametric model-checking.
-This extends both to LTL-style model-checkers for Promela-like languages
-@{cite "Cubicle" and "ByMC"} as well as process-algebra alikes 
-@{cite "AntoninoGR19" and "AntoninoGR16" and "BensalemGLNSY11"}. 
-However, the usual limitations persist: the translation to SMT is hardly certifiable and
-the solvers are still not able to handle non-linear computations; moreover, they fail
-to elaborate inductive proofs on data if necessary in refinement proofs. 
-
-Some systems involve approximation techniques in order to make the formal verification of 
-concurrent systems scalable; results are therefore inherently imprecise and require 
-meta-level arguments assuring their truth in a specific application context. 
-For example, in  @{cite "AntoninoGR19"}, the synchronization analysis  techniques try to 
-prove the unreachability of a system state by showing that components cannot agree 
-on the order or on the number of times they participate on system rules. 
-Even with such over-approximation, the finiteness restriction on the number of components 
-persists.
-
-Last but not least, SMT-based tools only focusing on bounded model-checking like
-@{cite "Kind2" and "JKind"} use k-induction and quite powerful invariant generation 
-techniques but are still far from scalable techniques. While it is difficult to make
-any precise argument on the scalability for HOL-CSP 2, we argue that we have no data-type 
-restrictions (events may have realvector-, function- or even process type) as well as
-restrictions on the structure of components. None of our paradigmatic examples can 
-be automatically proven with any of the discussed SMT techniques without restrictions.
-\<close>
-
-section*["conclusion",main_author="Some(@{docitem ''bu''}::author)"]\<open>Conclusion\<close>
-text\<open>We presented a formalisation of the most comprehensive semantic model for \<^csp>, a 'classical' 
-language for the specification and analysis of concurrent systems studied in a rich body of 
-literature. For this purpose, we ported @{cite "tej.ea:corrected:1997"} to a modern version
-of Isabelle, restructured the proofs, and extended the resulting theory of the language 
-substantially. The result HOL-CSP 2 has been submitted to the Isabelle AFP @{cite "HOL-CSP-AFP"}, 
-thus a fairly sustainable format accessible to other researchers and tools.
-
-We developed a novel set of deadlock - and livelock inference proof principles based on 
-classical and denotational characterizations. In particular, we formally investigated the relations
-between different refinement notions in the presence of deadlock - and livelock; an area where
-traditional \<^csp> literature skates over the nitty-gritty details. Finally, we demonstrated how to
-exploit these results for deadlock/livelock analysis of protocols.
-
-We put a large body of abstract \<^csp> laws and induction principles together to form
-concrete verification technologies for generalized classical problems, which have been considered
-so far from the perspective of data-independence or structural parametricity. The underlying novel
-principle of "trading rich structure against rich state" allows to convert processes 
-into classical transition systems for which established invariant techniques become applicable.
-
-Future applications of HOL-CSP 2 could comprise a combination to model checkers, where our theory
-with its derived rules is used to certify the output of a model-checker over \<^csp>. In our experience,
-generated labelled transition systems may be used to steer inductions or to construct
-the normalized processes \<open>P\<^sub>n\<^sub>o\<^sub>r\<^sub>m\<lbrakk>\<tau>\<^sub>,\<upsilon>\<rbrakk>\<close> automatically, thus combining efficient finite reasoning 
-over finite sub-systems with globally infinite systems in a logically safe way. 
-\<close>
-
-(*<*)
-subsection*[bib::bibliography]\<open>References\<close>
-
-close_monitor*[this]
-(*>*) 
-
-*)
 
 (*<*)
 end
